Change the representation of index so that every key must be mapped to a non-empty list of records Prove the type and semantic preservation of a transformation from list filtering to dictionary deletion

fiat2/src/fiat2/Index.v
@@ -1,5 +1,6 @@
 Require Import fiat2.Language fiat2.Interpret fiat2.Value fiat2.Examples fiat2.TypeSystem fiat2.TypeSound.
 Require Import List String ZArith Permutation.
+Import ListNotations.
 Require Import coqutil.Map.Interface coqutil.Word.Interface coqutil.Datatypes.Result.
 Import ResultMonadNotations.
 Require Import Sorted.
@@ -7,6 +8,62 @@ Require Import coqutil.Map.SortedListString.
 Require Import Ltac2.Ltac2 Ltac2.Control Ltac2.Constr.
 
 Set Default Proof Mode "Classic".
+
+Create HintDb fiat2_hints.
+
+Local Ltac invert_type_wf :=
+  lazymatch goal with
+  | H: type_wf (TList ?t) |- type_wf ?t => inversion H; clear H; subst
+  | H: type_wf (TOption ?t) |- type_wf ?t => inversion H; clear H; subst
+  | H: type_wf (TDict ?t _) |- type_wf ?t => inversion H; clear H; subst
+  | H: type_wf (TDict _ ?t) |- type_wf ?t => inversion H; clear H; subst
+  | H: type_wf (TRecord ?tl) |- Forall type_wf (List.map snd ?tl) => inversion H; clear H; subst
+  end.
+
+Lemma invert_TList_wf: forall t, type_wf (TList t) -> type_wf t.
+Proof.
+  intros. invert_type_wf; auto.
+Qed.
+
+Lemma invert_TOption_wf: forall t, type_wf (TOption t) -> type_wf t.
+Proof.
+  intros. invert_type_wf; auto.
+Qed.
+
+Lemma invert_TDict_wf_l: forall kt vt, type_wf (TDict kt vt) -> type_wf kt.
+Proof.
+  intros. invert_type_wf; auto.
+Qed.
+
+Lemma invert_TDict_wf_r: forall kt vt, type_wf (TDict kt vt) -> type_wf vt.
+Proof.
+  intros. invert_type_wf; auto.
+Qed.
+
+Lemma invert_TRecord_wf: forall tl, type_wf (TRecord tl) -> Forall type_wf (List.map snd tl).
+Proof.
+  intros. invert_type_wf; auto.
+Qed.
+
+Hint Resolve invert_TList_wf : fiat2_hints.
+Hint Resolve invert_TOption_wf : fiat2_hints.
+Hint Resolve invert_TDict_wf_l : fiat2_hints.
+Hint Resolve invert_TDict_wf_r : fiat2_hints.
+Hint Resolve invert_TRecord_wf : fiat2_hints.
+Hint Resolve type_of__type_wf : fiat2_hints.
+
+Local Ltac destruct_match :=
+  match goal with
+  | H: context[match ?x with _ => _ end] |- _ =>
+      let E := fresh "E" in
+      destruct x eqn:E
+  end.
+
+Local Ltac destruct_match_goal :=
+  let E := fresh "E" in
+  lazymatch goal with
+  | |- context[match ?x with _ => _ end] => destruct x eqn:E
+  end.
 
 Local Ltac iter_hyps tac :=
   let iter := ltac2:(tac |- List.iter (fun (h, _ , t) =>
@@ -21,6 +78,115 @@ Local Ltac rewrite_hyp_l h t :=
   try lazymatch t with
     | _ = _ => rewrite <- h in *
     end.
+
+Local Ltac invert_type_of :=
+  lazymatch goal with
+  | H: type_of _ _ (_ _) _ |- _ => inversion H; subst; clear H
+  | H: type_of_binop _ _ _ _ |- _ => inversion H; subst; clear H
+  end.
+
+Local Ltac invert_unop_binop_atom_ty :=
+  lazymatch goal with
+  | H: type_of_unop _ _ _ |- _ => inversion H; subst
+  | H: type_of_binop _ _ _ _ |- _ => inversion H; subst
+  | H: type_of_atom _ _ |- _ => inversion H; subst
+  end.
+
+Local Ltac invert_Forall :=
+  lazymatch goal with
+  | H: Forall _ (_ :: _) |- _ => inversion H; subst; clear H
+  end.
+
+Local Ltac invert_SSorted :=
+  lazymatch goal with
+  | H: StronglySorted _ (_ :: _) |- _ => inversion H; subst
+  end.
+
+Local Ltac invert_type_of_value :=
+  lazymatch goal with
+  | H: type_of_value ?v _ |- context[?v] => inversion H; subst; clear H
+  end.
+
+Local Ltac rewrite_map_get_put_hyp :=
+  multimatch goal with
+  | H: context[map.get (map.put _ ?x _) ?x] |- _ =>
+      rewrite map.get_put_same in H
+  | H: context[map.get (map.put _ _ _) _] |- _ =>
+      rewrite map.get_put_diff in H; try now (simpl in *; intuition)
+  end.
+
+Local Ltac rewrite_map_get_put_goal :=
+  multimatch goal with
+  | |- context[map.get (map.put _ ?x _) ?x] =>
+      rewrite map.get_put_same
+  | |- context[map.get (map.put _ _ _) _] =>
+      rewrite map.get_put_diff; try now (simpl in *; intuition)
+  end.
+
+
+Local Ltac clear_refl := lazymatch goal with H: ?x = ?x |- _ => clear H end.
+
+Local Ltac do_injection' h t :=
+  try lazymatch t with
+    | ?x _ = ?x _ => injection h; intros; subst
+    end.
+
+Local Ltac do_injection := iter_hyps do_injection'.
+
+Local Ltac destruct_subexpr :=
+  multimatch goal with
+  | e : expr |- _ => destruct e; auto; []
+  | o : unop |- _ => destruct o; auto; []
+  | o : binop |- _ => destruct o; auto; []
+  | a : atom |- _ => destruct a; auto; []
+  | t : option type |- _ => destruct t; auto; []
+  | l : list (expr * expr) |- _ => destruct l; auto; []
+  | l : list (string * expr) |- _ => destruct l; auto; []
+  | p : string * expr |- _ => destruct p; auto; []
+  | s : string |- _ => destruct s; auto; []
+  | a : Ascii.ascii |- _ => destruct a; auto; []
+  | b : bool |- _ => destruct b; auto; []
+  end.
+
+Local Ltac apply_Forall_In :=
+  lazymatch goal with
+  | H1: Forall _ ?l, H2: In _ ?l |- _ => eapply List.Forall_In in H1; eauto
+  end.
+
+Local Ltac rewrite_expr_value :=
+  lazymatch goal with
+  | E: VList _ = ?e |- context[?e] => rewrite <- E
+  | E: VList _ = ?e, H: context[?e] |- _ => rewrite <- E in H
+  end.
+
+Local Ltac apply_type_sound e :=
+  lazymatch goal with
+  | H: type_of _ _ e _ |- _ =>
+      let H' := fresh "H'" in
+      eapply type_sound in H as H'; eauto; try inversion H'; subst; auto
+  end.
+
+Local Ltac rewrite_interp_fold_expr :=
+  lazymatch goal with
+  | H: interp_expr _ _ (fold_expr _ ?e) = _ |- context[fold_expr _ ?e] =>
+      rewrite H; clear H
+  end.
+
+Local Ltac get_update_same_diff x y :=
+  let E := fresh "E" in
+  destruct (String.eqb x y) eqn:E;
+  [ rewrite eqb_eq in E; subst; repeat rewrite Properties.map.get_update_same
+  | rewrite eqb_neq in E; repeat rewrite Properties.map.get_update_diff ]; auto.
+
+Local Ltac get_put_same_diff x y :=
+  let E := fresh "E" in
+  destruct (String.eqb x y) eqn:E;
+  [ rewrite eqb_eq in E; subst; repeat rewrite map.get_put_same
+  | rewrite eqb_neq in E; repeat rewrite map.get_put_diff ]; auto.
+
+Local Ltac invert_Forall2 := lazymatch goal with H: Forall2 _ _ _ |- _ => inversion H; subst; clear H end.
+
+Local Ltac rewrite_l_to_r := lazymatch goal with H: ?x = _ |- context[?x] => rewrite H end.
 
 Section fold_command.
   Context (f : command -> command).
@@ -39,24 +205,300 @@ Section fold_command.
       end.
 End fold_command.
 
-(* Materialize tbl (expected to be a list of records) into an index over attr *)
-Definition list_to_idx (attr : string) (tbl : expr) : expr :=
-  EFold tbl (EDict nil) "tup" "acc"
-    (EInsert (EVar "acc") (EAccess (EVar "tup") attr)
-       (EBinop OCons (EVar "tup")
-          (EOptMatch (ELookup (EVar "acc") (EAccess (EVar "tup") attr))
-             (EAtom (ANil None))
-             "x"%string (EVar "x")))).
+Open Scope string_scope.
 
-(* Inverse of tbl_to_idx, expecting idx to be a dict
-   Require the index keys in idx to match the attr values in the records *)
-Definition idx_to_list (idx : expr) : expr :=
-  EDictFold idx (EAtom (ANil None)) "k" "v" "acc" (EBinop OConcat (EVar "v") (EVar "acc")).
+Definition epair (e1 e2 : expr) := ERecord [("0", e1); ("1", e2)].
+Definition ofst (e : expr) : expr := EAccess e "0".
+Definition osnd (e : expr) : expr := EAccess e "1".
+Definition enil := EAtom (ANil None).
+Definition econs (e1 e2 : expr) := EBinop OCons e1 e2.
+Definition cons_to_fst (e1 e2 : expr) :=
+  epair (econs e1 (ofst e2)) (osnd e2).
+
+Fixpoint is_NoDup {A} (l : list A) : Prop :=
+  match l with
+  | nil => True
+  | x :: l => ~ In x l /\ is_NoDup l
+  end.
+
+Lemma In_access_record : forall A l attr, In attr (List.map fst l) -> exists (x : A), access_record l attr = Success x.
+Proof.
+  induction l; simpl; intros.
+  - intuition.
+  - destruct a; simpl in *. destruct (eqb attr s) eqn:E.
+    + exists a. reflexivity.
+    + rewrite eqb_neq in *. intuition. congruence.
+Qed.
+
+Lemma access_record_type_wf : forall rt attr t,
+    type_wf (TRecord rt) ->
+    access_record rt attr = Success t ->
+    type_wf t.
+Proof.
+  intros * H_ty H. apply access_record_sound in H. apply in_map with (f:=snd) in H; simpl in H.
+  inversion H_ty; subst. apply_Forall_In.
+Qed.
+
+
+Lemma In_map_ext : forall A B (f g : A -> B) l, (forall x, In x l -> f x = g x) -> List.map f l = List.map g l.
+Proof.
+  intros * H. induction l; simpl; auto.
+  f_equal; [ apply H | apply IHl ]; intuition.
+Qed.
+
+Lemma Permutation_filter : forall A (l l' : list A), Permutation l l' -> forall f, Permutation (filter f l) (filter f l').
+Proof.
+  induction l; intros.
+  - apply Permutation_nil in H. subst. auto.
+  - apply Permutation_sym in H as H'. apply Permutation_vs_cons_inv in H'.
+    repeat lazymatch goal with H: exists _, _ |- _ => destruct H end.
+    subst. rewrite filter_app. simpl; destruct (f a).
+    1: apply Permutation_cons_app.
+    all: rewrite <- filter_app.
+    all: apply Permutation_cons_app_inv in H; auto.
+Qed.
+
+Lemma Permutation_flat_map : forall A B (f g : A -> list B),
+  forall l l', (forall x, In x l -> Permutation (f x) (g x)) ->
+               Permutation l l' ->
+               Permutation (flat_map f l) (flat_map g l').
+Proof.
+  intros * H_fg. generalize dependent l'. induction l; simpl; intros l' H.
+  - apply Permutation_nil in H; subst; auto.
+  - apply Permutation_sym in H as H'. apply Permutation_vs_cons_inv in H'.
+    repeat lazymatch goal with H: exists _, _ |- _ => destruct H end. subst.
+    rewrite flat_map_app. simpl. pose proof H_fg a as H_a.
+    assert (H_a_in: In a (a :: l)). { intuition. } apply H_a in H_a_in as H_p.
+    destruct (f a) eqn:E.
+    + simpl. apply Permutation_nil in H_p.
+      rewrite H_p; simpl. rewrite <- flat_map_app.
+      apply Permutation_cons_app_inv in H. intuition.
+    + eapply perm_trans. 2: apply Permutation_app_swap_app.
+      apply Permutation_app; auto. rewrite <- flat_map_app. apply IHl.
+      2: apply Permutation_cons_app_inv in H.
+      all: intuition.
+Qed.
+
+Lemma imp_pre_true : forall A B, A -> (A -> B) -> A /\ B.
+Proof. intuition. Qed.
+
+Section __.
+  Context (tbl attr : string).
+
+  (* is_inv stands for whether the context is invariant to Permutations of the current expr's output *)
+  Definition unop_is_inv (is_inv : bool) (o : unop) : bool :=
+    match o with
+    | OLength => true
+    | _ => false
+    end.
+
+  Definition binop_is_inv (is_inv : bool) (o : binop) : bool * bool :=
+    match o with
+    | OCons => (false, is_inv)
+    | _ => (false, false)
+    end.
+
+  Fixpoint can_transf_to_idx'' (is_inv : bool) (e : expr) : bool :=
+    match e with
+    | EVar _ | EAtom _ => true
+    | ELoc x => negb (String.eqb x tbl) || is_inv
+    | EUnop o e => can_transf_to_idx'' (unop_is_inv is_inv o) e
+    | EBinop o e1 e2 => let '(b1, b2) := binop_is_inv is_inv o in
+                        can_transf_to_idx'' b1 e1 && can_transf_to_idx'' b2 e2
+    | EIf e1 e2 e3 => can_transf_to_idx'' false e1 && can_transf_to_idx'' is_inv e2 && can_transf_to_idx'' is_inv e3
+    | ELet e1 x e2 => can_transf_to_idx'' false e1 && can_transf_to_idx'' is_inv e2
+    | EFlatmap e1 x e2 => can_transf_to_idx'' is_inv e1 && can_transf_to_idx'' is_inv e2
+    | EFold e1 e2 x y e3 => can_transf_to_idx'' false e1 && can_transf_to_idx'' false e2 && can_transf_to_idx'' false e3
+    | ERecord l => forallb (fun p => can_transf_to_idx'' false (snd p)) l
+    | EAccess e s => can_transf_to_idx'' false e
+    | EDict l => forallb (fun p => (can_transf_to_idx'' false (fst p) && can_transf_to_idx'' false (snd p))%bool) l
+    | EInsert d k v => can_transf_to_idx'' false d && can_transf_to_idx'' false k && can_transf_to_idx'' false v
+    | EDelete d k => can_transf_to_idx'' false d && can_transf_to_idx'' false k
+    | ELookup d k => can_transf_to_idx'' false d && can_transf_to_idx'' false k
+    | EOptMatch e e_none x e_some => can_transf_to_idx'' false e && can_transf_to_idx'' is_inv e_none && can_transf_to_idx'' is_inv e_some
+    | EDictFold d e0 k v acc e => can_transf_to_idx'' false d && can_transf_to_idx'' false e0 && can_transf_to_idx'' false e
+    | ESort l => can_transf_to_idx'' true l
+    | EFilter l x p => can_transf_to_idx'' is_inv l && can_transf_to_idx'' false p
+    | EJoin l1 l2 x1 x2 p r => can_transf_to_idx'' is_inv l1 && can_transf_to_idx'' is_inv l2 && can_transf_to_idx'' false p && can_transf_to_idx'' false r
+    | EProj l x r => can_transf_to_idx'' is_inv l && can_transf_to_idx'' false r
+    end.
+
+  Fixpoint can_transf_to_idx' (c : command) : bool :=
+    match c with
+    | CSkip => true
+    | CSeq c1 c2 => can_transf_to_idx' c1 && can_transf_to_idx' c2
+    | CLet e x c => can_transf_to_idx'' false e && can_transf_to_idx' c
+    | CLetMut e x c => negb (String.eqb x tbl) && can_transf_to_idx'' false e && can_transf_to_idx' c
+    | CAssign x e => can_transf_to_idx'' false e
+    | CIf e c1 c2 => can_transf_to_idx'' false e && can_transf_to_idx' c1 && can_transf_to_idx' c2
+    | CForeach e x c => can_transf_to_idx'' false e && can_transf_to_idx' c
+    end.
+
+  Definition can_transf_to_idx (c : command) : bool :=
+    match c with
+    | CLetMut (EAtom (ANil (Some (TRecord rt)))) x c =>
+        String.eqb x tbl &&
+          inb String.eqb attr (List.map fst rt) &&
+          can_transf_to_idx' c
+    | _ => false
+    end.
+End __.
 
 Section WithWord.
   Context {width: Z} {word: word.word width}.
   Context {word_ok: word.ok word}.
   Local Notation value := (value (word := word)).
+
+  (* ??? TODO: move *)
+  Lemma value_eqb_refl : forall (v : value), value_eqb v v = true.
+  Proof.
+    unfold value_eqb. intros; rewrite value_compare_refl; reflexivity.
+  Qed.
+
+  Fixpoint concat_VList_V (l : list value) :=
+    match l with
+    | VRecord l' :: l => match record_proj "0" l' with
+                         | VList vl => (vl ++ (record_proj "1" l' :: concat_VList_V l))%list
+                         | _ => nil
+                         end
+    | _ => nil
+    end.
+
+  Definition has_index_entry_shape (p : value * value) :=
+    match snd p with
+    | VRecord r =>
+        match record_proj "0" r with
+        | VList _ => True | _ => False end
+    | _ => False end.
+
+  Definition vcons_to_fst (v p : value) : value :=
+    VRecord [("0", match p with
+                   | VRecord p =>
+                       match record_proj "0" p with
+                       | VList l => VList (v :: l)
+                       | _ => VUnit
+                       end
+                   | _ => VUnit
+                   end);
+             ("1", match p with
+                   | VRecord p => record_proj "1" p
+                   | _ => VUnit
+                   end)].
+
+  Local Coercion is_true : bool >-> Sortclass.
+
+  Lemma dict_insert_preserve_SSorted : forall d k v,
+      StronglySorted (dict_entry_leb (word:=word)) d ->
+      StronglySorted dict_entry_leb (dict_insert k v d).
+  Proof.
+    induction d; intros; simpl.
+    - repeat constructor.
+    - destruct a. inversion H; subst. unfold value_ltb, value_eqb.
+      lazymatch goal with
+      | |- context[value_compare ?a ?b] => destruct (value_compare a b) eqn:E
+      end.
+      + constructor; auto. rewrite Forall_forall in *.
+        unfold dict_entry_leb in *; simpl in *. apply value_compare_Eq_eq in E; subst; auto.
+      + constructor; auto. rewrite Forall_forall in *; intros. destruct x.
+        unfold dict_entry_leb, value_leb, leb_from_compare in *; simpl in *.
+        destruct H0.
+        * inversion H0; subst; rewrite E; auto.
+        * apply H3 in H0; simpl in H0. destruct (value_compare v0 v2) eqn:E'; intuition.
+          1: { apply value_compare_Eq_eq in E'; subst; rewrite E; trivial. }
+          erewrite value_compare_trans; eauto.
+      + constructor; auto. rewrite Forall_forall; intros x H_in.
+        apply dict_insert_incl in H_in.
+        unfold dict_entry_leb, value_leb, leb_from_compare in *; simpl in *.
+        inversion H_in; subst.
+        * simpl. rewrite value_compare_antisym. rewrite E. auto.
+        * eapply List.Forall_In in H3; eauto.
+  Qed.
+
+  Lemma dict_lookup_Lt : forall d k,
+      StronglySorted dict_entry_leb d ->
+      (forall p, In p d -> value_compare k (fst p) = Lt) ->
+      dict_lookup (word:=word) k d = None.
+  Proof.
+    intros. induction d; auto.
+    simpl. destruct a; simpl in *.
+    destruct (value_eqb k v) eqn:E.
+    - unfold value_eqb in *. pose proof (H0 (v, v0)).
+      intuition; simpl in *. rewrite H1 in E; discriminate.
+    - apply IHd; inversion H; auto.
+  Qed.
+
+  Lemma Forall_dict_lookup : forall P d k v,
+      Forall P d -> dict_lookup (width:=width) k d = Some v -> P (k, v).
+  Proof.
+    intros * H_P H. induction d; simpl in H; try congruence.
+    destruct a. inversion H_P; subst.
+    lazymatch goal with
+    | H: context[value_eqb ?a ?b] |- _ => destruct (value_eqb a b) eqn:E
+    end.
+    1: apply value_eqb_eq in E; subst; do_injection; auto.
+    1: apply IHd; auto.
+  Qed.
+
+  Lemma dict_insert_lookup_Permutation :
+    forall k d v, Forall has_index_entry_shape d ->
+                  StronglySorted dict_entry_leb d ->
+                  Permutation
+                    (concat_VList_V
+                       (List.map snd
+                          (dict_insert k
+                             match dict_lookup k d with
+                             | Some p => vcons_to_fst v p
+                             | None =>
+                                 VRecord [("0", VList []); ("1", v)]
+                             end d)))
+                    (v :: (concat_VList_V (List.map snd d))).
+  Proof.
+    unfold has_index_entry_shape; intros * H H_SSorted.
+    induction d; simpl; auto.
+    destruct a; simpl. inversion H; subst; simpl in *.
+    destruct v1; intuition.
+    unfold value_eqb, value_ltb. destruct (value_compare k v0) eqn:E; cbn; auto.
+    all: destruct (record_proj "0" l); intuition.
+    all: inversion H_SSorted; subst.
+    - rewrite dict_lookup_Lt; auto. intros p H_in. apply_Forall_In.
+      unfold dict_entry_leb, value_leb, leb_from_compare in *; simpl in *.
+      destruct (value_compare v0 (fst p)) eqn:E'; try congruence.
+      + apply value_compare_Eq_eq in E'; subst; auto.
+      + eapply value_compare_trans; eauto.
+    - assert (H_Permu: forall A (l : list A) u v xl yl, Permutation xl (v :: yl) -> Permutation (l ++ u :: xl) (v :: l ++ u :: yl)).
+      { clear. intros.
+        replace (v :: l ++ u :: yl) with ((v :: nil) ++ l ++ u :: yl)%list; auto.
+        eapply perm_skip with (x:=u), Permutation_sym, perm_trans in H.
+        2: apply perm_swap.
+        eapply perm_trans. 2: eapply Permutation_app_swap_app. simpl.
+        auto using Permutation_app, Permutation_sym. }
+      auto.
+  Qed.
+
+  Lemma Permutation_SSorted_eq : forall l l',
+      Permutation l l' ->
+      StronglySorted (value_leb (word:=word)) l ->
+      StronglySorted value_leb l' ->
+      l = l'.
+  Proof.
+    induction l; intros l' H H_sort H_sort'.
+    - apply Permutation_nil in H; congruence.
+    - destruct l'.
+      1: apply Permutation_sym, Permutation_nil in H; discriminate.
+      inversion H_sort; inversion H_sort'; subst.
+      apply Permutation_in with (x:=a) in H as H_in; intuition.
+      apply Permutation_sym in H as H'.
+      apply Permutation_in with (x:=v) in H' as H_in'; intuition.
+      inversion H_in; inversion H_in'; subst.
+      1-3: f_equal; apply IHl; auto; eapply Permutation_cons_inv; eauto.
+      eapply List.Forall_In in H3, H7; eauto.
+      apply value_leb_antisym in H3; auto; subst. f_equal.
+      apply IHl; auto. eapply Permutation_cons_inv; eauto.
+  Qed.
+
+  (* An index is a dictionary with each of its keys mapped to at least one row of the table *)
+  Definition index_type (kt : type) (rt : list (string * type)) :=
+    TDict kt (TRecord [("0", TList (TRecord rt)); ("1", TRecord rt)]).
 
   Section WithMap.
     Context {tenv: map.map string type} {tenv_ok: map.ok tenv}.
@@ -65,550 +507,28 @@ Section WithWord.
     Definition gallina_list_to_idx attr (l : list value) :=
       fold_right
         (fun v acc => match v with
-                      | VRecord v => dict_insert (record_proj attr v)
-                                       (match dict_lookup (record_proj attr v) acc with
-                                        | Some l' => match l' with
-                                                     | VList l' => VList (VRecord v :: l')
-                                                     | _ => VUnit
-                                                     end
-                                        | _ => VList (VRecord v :: nil)
-                                        end) acc
-           | _ => nil
-           end) nil l.
+                      | VRecord v =>
+                          dict_insert (record_proj attr v)
+                            (match dict_lookup (record_proj attr v) acc with
+                             | Some p => vcons_to_fst (VRecord v) p
+                             | None => VRecord [("0", VList nil); ("1", VRecord v)]
+                             end) acc
+                      | _ => nil
+                      end) nil l.
 
     Definition gallina_idx_to_list (d : list (value * value)) :=
       fold_right
         (fun v acc => match snd v with
-                      | VList v => app v acc
+                      | VRecord p => match record_proj "0" p with
+                                     | VList l => (l ++ (record_proj "1" p :: acc))%list
+                                     | _ => nil
+                                     end
                       | _ => nil
                       end)
         nil d.
 
-    Lemma fiat2_gallina_list_to_idx : forall (Gstore Genv : tenv) (store env : locals) tbl attr l rt,
-        type_of Gstore Genv tbl (TList (TRecord rt)) ->
-        tenv_wf Gstore -> tenv_wf Genv ->
-        locals_wf Gstore store -> locals_wf Genv env ->
-        In attr (List.map fst rt) ->
-        interp_expr store env tbl = VList l ->
-        interp_expr store env (list_to_idx attr tbl) = VDict (gallina_list_to_idx attr l).
-    Proof.
-      intros. simpl. rewrite H5. eapply type_sound in H; eauto; subst.
-      rewrite H5 in H; clear tbl H5.
-      erewrite In_fold_right_ext with (P := fun v => match v with VDict _ => True | _ => False end)
-                                      (g := (fun x y =>
-                                               match x, y with
-                                               | VRecord l1, VDict l0 =>
-                                                   VDict
-                                                     (dict_insert (record_proj attr l1)
-                                                        match
-                                                          match dict_lookup (record_proj attr l1) l0 with
-                                                          | Some v =>
-                                                              v
-                                                          | None => VList nil
-                                                          end
-                                                        with
-                                                        | VList l2 => VList (VRecord l1 :: l2)
-                                                        | _ => VUnit
-                                                        end l0)
-                                               | _ , _=> VUnit
-                                               end)).
-      3:{
-        intros.
-        unfold get_local; rewrite !map.get_put_same.
-        rewrite !map.get_put_diff by congruence. rewrite !map.get_put_same.
-        destruct a; intuition.
-        inversion H; subst. eapply List.Forall_In in H9; eauto.
-        inversion H9; subst.
-        destruct (dict_lookup (record_proj attr l1) l0); try reflexivity.
-        rewrite !map.get_put_same. reflexivity.
-      }
-      2: trivial.
-      induction l; simpl; auto.
-      inversion H; subst. inversion H7; subst. inversion H8; subst.
-      rewrite IHl.
-      2:{ constructor; auto. }
-      f_equal. f_equal.
-      destruct (dict_lookup (record_proj attr l0) (gallina_list_to_idx attr l)); auto.
-    Qed.
-
-    Lemma fiat2_gallina_idx_to_list : forall (Gstore Genv : tenv) (store env : locals) idx l kt t,
-        type_of Gstore Genv idx (TDict kt (TList t)) ->
-        tenv_wf Gstore -> tenv_wf Genv ->
-        locals_wf Gstore store -> locals_wf Genv env ->
-        interp_expr store env idx = VDict l ->
-        interp_expr store env (idx_to_list idx) = VList (gallina_idx_to_list l).
-    Proof.
-      intros. simpl. eapply type_sound in H; eauto.
-      rewrite H4 in *. inversion H; subst. clear H4 idx.
-      erewrite In_fold_right_ext with (P := fun v => match v with VList _ => True | _ => False end)
-                                      (g := fun b a => match snd b with
-                                                       | VList a0 => match a with
-                                                                     | VList b0 => VList (a0 ++ b0)
-                                                                     | _ => VUnit
-                                                                     end
-                                                       | _ => VUnit
-                                                       end).
-      3:{ intros. unfold get_local; rewrite !map.get_put_same.
-          rewrite !map.get_put_diff by congruence. rewrite !map.get_put_same.
-          eapply List.Forall_In in H10; eauto; intuition.
-          inversion H7; subst. destruct a; intuition.
-      }
-      2: trivial.
-      induction l; simpl; auto. simpl in *; inversion H10; inversion H11; inversion H12; subst.
-      rewrite IHl; auto.
-      2: constructor; auto.
-      intuition. inversion H5; subst. reflexivity.
-    Qed.
-
-    Fixpoint concat_VList (l : list value) :=
-      match l with
-      | VList l' :: l => app l' (concat_VList l)
-      | _ => nil
-      end.
-
-    Local Coercion is_true : bool >-> Sortclass.
-
-    Lemma dict_lookup_Lt : forall d k,
-        StronglySorted dict_entry_leb d ->
-        (forall p, In p d -> value_compare k (fst p) = Lt) ->
-        dict_lookup (word:=word) k d = None.
-    Proof.
-      intros. induction d; auto.
-      simpl. destruct a; simpl in *.
-      destruct (value_eqb k v) eqn:E.
-      - unfold value_eqb in *. pose proof (H0 (v, v0)).
-        intuition; simpl in *. rewrite H1 in E; discriminate.
-      - apply IHd; inversion H; auto.
-    Qed.
-
-    Lemma dict_insert_lookup_Permutation :
-      forall k d v, Forall (fun v => match snd v with VList _ => True | _ => False end) d ->
-                    StronglySorted dict_entry_leb d ->
-                    Permutation
-                      (concat_VList
-                         (List.map snd
-                            (dict_insert k
-                               match dict_lookup k d with
-                               | Some (VList l) => VList (v :: l)
-                               | None => VList (v :: nil)
-                               | _ => VUnit
-                               end d)))
-                      (v :: (concat_VList (List.map snd d))).
-    Proof.
-      intros. induction d; simpl; auto.
-      destruct a; simpl. inversion H; subst; simpl in *. destruct v1; intuition.
-      unfold value_eqb, value_ltb. destruct (value_compare k v0) eqn:E; simpl; auto.
-      - inversion H0; subst. rewrite dict_lookup_Lt; auto. intros p H_in.
-        eapply List.Forall_In in H7; eauto. unfold dict_entry_leb, value_leb, leb_from_compare in H7; simpl in H7.
-        destruct (value_compare v0 (fst p)) eqn:E'; try congruence.
-        + apply value_compare_Eq_eq in E'; subst; auto.
-        + eapply value_compare_trans; eauto.
-      - assert (forall xl v yl, Permutation xl (v :: yl) -> Permutation (l ++ xl) (v :: l ++ yl)).
-        { clear. intros. replace (v :: l ++ yl) with ((v :: nil) ++ l ++ yl); auto.
-          eapply perm_trans.
-          2: eapply Permutation_app_swap_app. simpl.
-          apply Permutation_app; auto. }
-        apply H2; apply H1; inversion H0; auto.
-    Qed.
-
-    Lemma dict_lookup_VList : forall k l,
-        Forall (fun p => match snd p with VList _ => True | _ => False end) l ->
-        match dict_lookup (word:=word) k l with Some (VList _) | None => True | _ => False end.
-    Proof.
-      intros; induction l; simpl; auto.
-      destruct a. destruct (value_eqb k v); auto.
-      - inversion H; subst; auto.
-      - apply IHl. inversion H; intuition.
-    Qed.
-
-    Lemma gallina_list_to_idx_VList : forall l attr rt,
-        Forall (fun v => type_of_value v (TRecord rt)) l ->
-        In attr (List.map fst rt) ->
-        Forall (fun p => match snd p with VList _ => True | _ => False end) (gallina_list_to_idx attr l).
-    Proof.
-      intros; induction l; simpl; auto.
-      inversion H; subst. inversion H3; subst.
-      rewrite Forall_forall; intros x H_in. apply dict_insert_incl in H_in.
-      inversion H_in; subst; simpl.
-      - apply IHl in H4. eapply dict_lookup_VList with (k:=(record_proj attr l0)) in H4.
-        lazymatch goal with |- context[dict_lookup ?k ?d] => destruct (dict_lookup k d) end; intuition. destruct v; intuition.
-      - apply IHl in H4. rewrite Forall_forall in H4. apply H4; auto.
-    Qed.
-
-    Lemma dict_insert_preserve_SSorted : forall d k v,
-        StronglySorted (dict_entry_leb (word:=word)) d ->
-        StronglySorted dict_entry_leb (dict_insert k v d).
-    Proof.
-      induction d; intros; simpl.
-      - repeat constructor.
-      - destruct a. inversion H; subst. unfold value_ltb, value_eqb. destruct (value_compare k v0) eqn:E.
-        + constructor; auto. rewrite Forall_forall in *.
-          unfold dict_entry_leb in *; simpl in *. apply value_compare_Eq_eq in E; subst; auto.
-        + constructor; auto. rewrite Forall_forall in *; intros. destruct x.
-          unfold dict_entry_leb, value_leb, leb_from_compare in *; simpl in *.
-          destruct H0.
-          * inversion H0; subst; rewrite E; auto.
-          * apply H3 in H0; simpl in H0. destruct (value_compare v0 v2) eqn:E'; intuition.
-            1: { apply value_compare_Eq_eq in E'; subst; rewrite E; trivial. }
-            erewrite value_compare_trans; eauto.
-        + constructor; auto. rewrite Forall_forall; intros x H_in.
-          apply dict_insert_incl in H_in.
-          unfold dict_entry_leb, value_leb, leb_from_compare in *; simpl in *.
-          inversion H_in; subst.
-          * simpl. rewrite value_compare_antisym. rewrite E. auto.
-          * eapply List.Forall_In in H3; eauto.
-    Qed.
-
-    Lemma gallina_list_to_idx_SSorted : forall l attr rt,
-        Forall (fun v => type_of_value v (TRecord rt)) l ->
-        In attr (List.map fst rt) ->
-        StronglySorted dict_entry_leb (gallina_list_to_idx attr l).
-    Proof.
-      intros; induction l; simpl; try constructor.
-      inversion H; subst. inversion H3; subst.
-      apply dict_insert_preserve_SSorted; auto.
-    Qed.
-
-    Lemma gallina_list_to_idx_Permutation : forall attr l rt,
-        Forall (fun v => type_of_value v (TRecord rt)) l ->
-        In attr (List.map fst rt) ->
-        Permutation (concat_VList (List.map snd (gallina_list_to_idx attr l))) l.
-    Proof.
-      intros. induction H; intuition.
-      simpl in *. inversion H; subst. eapply perm_trans.
-      - eapply dict_insert_lookup_Permutation.
-        + eapply gallina_list_to_idx_VList; eauto.
-        + eapply gallina_list_to_idx_SSorted; eauto.
-      - constructor; auto.
-    Qed.
-
-    Lemma gallina_list_to_idx_to_list : forall attr l rt ,
-        Forall (fun v => type_of_value v (TRecord rt)) l ->
-        In attr (List.map fst rt) ->
-        Permutation (gallina_idx_to_list (gallina_list_to_idx attr l)) l.
-    Proof.
-      intros.
-      assert (forall l, Forall (fun v => match snd v with VList _ => True | _ => False end) l -> gallina_idx_to_list l = concat_VList (List.map snd l)).
-      { induction l0; simpl; intros; auto. inversion H1; subst. destruct (snd a); intuition. congruence. }
-      pose proof (gallina_list_to_idx_Permutation _ _ _ H H0). rewrite <- H1 in H2; auto.
-      revert H H0; clear. intro; rewrite Forall_forall. induction l; simpl; intros.
-      - intuition.
-      - inversion H; subst. inversion H4; subst.
-        apply dict_insert_incl in H1 as H1'; inversion H1'; subst.
-        2: apply IHl; auto.
-        simpl. destruct (dict_lookup (record_proj attr l0) (gallina_list_to_idx attr l)) eqn:E; intuition.
-        destruct v; intuition. all: eapply gallina_list_to_idx_VList with (l:=l) in H0; eauto; intuition; eapply dict_lookup_VList in H0; erewrite E in H0; intuition.
-    Qed.
-
-    Lemma In_access_record : forall A l attr, In attr (List.map fst l) -> exists (x : A), access_record l attr = Success x.
-    Proof.
-      induction l; simpl; intros.
-      - intuition.
-      - destruct a; simpl in *. destruct (eqb attr s) eqn:E.
-        + exists a. reflexivity.
-        + rewrite eqb_neq in *. intuition. congruence.
-    Qed.
-
-    Lemma fiat2_gallina_list_to_idx_to_list : forall (Gstore Genv : tenv) (store env : locals) l attr tbl rt,
-        type_of Gstore Genv tbl (TList (TRecord rt)) ->
-        tenv_wf Gstore -> tenv_wf Genv ->
-        locals_wf Gstore store -> locals_wf Genv env ->
-        In attr (List.map fst rt) ->
-        interp_expr store env tbl = VList l ->
-        interp_expr store env (idx_to_list (list_to_idx attr tbl)) =
-          VList (gallina_idx_to_list (gallina_list_to_idx attr l)).
-    Proof.
-      intros.
-      apply In_access_record in H4 as Ht.
-      destruct Ht as [t Ht].
-      intros. eapply fiat2_gallina_idx_to_list with (Gstore:=Gstore) (kt:=t); eauto.
-      2:{ eapply fiat2_gallina_list_to_idx with (Gstore:=Gstore); eauto. }
-      apply type_of__type_wf in H as H_wf; auto. inversion H_wf; subst. inversion H7; subst.
-      repeat (try econstructor; try erewrite map.get_put_same; try erewrite map.get_put_diff; try congruence; eauto).
-      eapply Forall_access_record; eauto.
-    Qed.
-
-    Lemma list_to_idx_to_list :
-      forall attr tbl (Gstore Genv : tenv) (store env : locals) rt,
-        type_of Gstore Genv tbl (TList (TRecord rt)) ->
-        tenv_wf Gstore -> tenv_wf Genv ->
-        locals_wf Gstore store -> locals_wf Genv env ->
-        In attr (List.map fst rt) ->
-        exists l l', interp_expr store env (idx_to_list (list_to_idx attr tbl)) = VList l /\
-                       interp_expr store env tbl = VList l' /\
-                       Permutation l l'.
-    Proof.
-      intros. eapply type_sound in H as H'; eauto. inversion H'; subst. symmetry in H5.
-      eapply fiat2_gallina_list_to_idx_to_list with (attr:=attr) in H5 as H5'; eauto. repeat eexists; eauto.
-      eapply gallina_list_to_idx_to_list; eauto.
-    Qed.
-
-    Lemma Permutation_SSorted_eq : forall l l',
-        Permutation l l' ->
-        StronglySorted (value_leb (word:=word)) l ->
-        StronglySorted value_leb l' ->
-        l = l'.
-    Proof.
-      induction l; intros l' H H_sort H_sort'.
-      - apply Permutation_nil in H; congruence.
-      - destruct l'.
-        1: apply Permutation_sym, Permutation_nil in H; discriminate.
-        inversion H_sort; inversion H_sort'; subst.
-        apply Permutation_in with (x:=a) in H as H_in; intuition.
-        apply Permutation_sym in H as H'.
-        apply Permutation_in with (x:=v) in H' as H_in'; intuition.
-        inversion H_in; inversion H_in'; subst.
-        1-3: f_equal; apply IHl; auto; eapply Permutation_cons_inv; eauto.
-        eapply List.Forall_In in H3, H7; eauto.
-        apply value_leb_antisym in H3; auto; subst. f_equal.
-        apply IHl; auto. eapply Permutation_cons_inv; eauto.
-    Qed.
-
-    Lemma ESort_Permutation_inv : forall (store env : locals) l l' vl vl',
-        interp_expr store env l = VList vl ->
-        interp_expr store env l' = VList vl' ->
-        Permutation vl vl' ->
-        interp_expr store env (ESort l) = interp_expr store env (ESort l').
-    Proof.
-      intros store env l l' vl vl' E E' H. simpl.
-      rewrite E, E'. f_equal.
-      apply Permutation_SSorted_eq.
-      2,3: apply StronglySorted_value_sort.
-      eapply perm_trans. 2:apply Permuted_value_sort.
-      eapply perm_trans. 2:apply H.
-      apply Permutation_sym, Permuted_value_sort.
-    Qed.
-
-    Lemma list_to_idx_preserve_ty : forall Gstore Genv tbl rt attr,
-        tenv_wf Gstore -> tenv_wf Genv ->
-        In attr (List.map fst rt) ->
-        type_of Gstore Genv tbl (TList (TRecord rt)) ->
-        type_of Gstore Genv (list_to_idx attr tbl) (TDict (get_attr_type rt attr) (TList (TRecord rt))).
-    Proof.
-      intros. eapply type_of__type_wf in H2 as H_wf; auto. inversion H_wf; subst.
-      inversion H4; subst. repeat econstructor; eauto.
-      all: repeat (try rewrite map.get_put_same; try rewrite map.get_put_diff; try congruence); eauto.
-      all: unfold get_attr_type; apply In_access_record in H1 as [t Ht]; rewrite Ht; auto.
-      apply access_record_sound in Ht. apply in_map with (f:=snd) in Ht. eapply List.Forall_In in H7; eauto.
-    Qed.
-
-    Lemma idx_to_list_preserve_ty : forall Gstore Genv idx kt t,
-        tenv_wf Gstore -> tenv_wf Genv ->
-        type_of Gstore Genv idx (TDict kt (TList t)) ->
-        type_of Gstore Genv (idx_to_list idx) (TList t).
-    Proof.
-      intros. eapply type_of__type_wf in H1 as H_wf; auto. inversion H_wf; subst. inversion H5; subst.
-      repeat econstructor; eauto.
-      all: repeat (try rewrite map.get_put_same; try rewrite map.get_put_diff; try congruence).
-      Qed.
-
-    Definition idx_read_to_list_read (tbl : string) (e : expr) :=
-      match e with
-      | ELoc tbl' => if String.eqb tbl tbl'
-                     then idx_to_list (ELoc tbl)
-                     else e
-      | _ => e
-      end.
-
-    Definition list_write_to_idx_write (tbl attr : string) (c : command) :=
-      match c with
-      | CAssign tbl' e =>
-          if String.eqb tbl tbl'
-          then CAssign tbl (list_to_idx attr e)
-          else c
-      | _ => c
-      end.
-
-    Section __.
-      Context (tbl attr : string).
-
-      (* is_inv stands for whether the context is invariant to Permutations of the current expr's output *)
-      Definition unop_is_inv (is_inv : bool) (o : unop) : bool :=
-        match o with
-        | OLength => true
-        | _ => false
-        end.
-
-      Definition binop_is_inv (is_inv : bool) (o : binop) : bool * bool :=
-        match o with
-        | OCons => (false, is_inv)
-        | _ => (false, false)
-        end.
-
-      Fixpoint can_transf_to_idx'' (is_inv : bool) (e : expr) : bool :=
-        match e with
-        | EVar _ | EAtom _ => true
-        | ELoc x => negb (String.eqb x tbl) || is_inv
-        | EUnop o e => can_transf_to_idx'' (unop_is_inv is_inv o) e
-        | EBinop o e1 e2 => let '(b1, b2) := binop_is_inv is_inv o in
-                            can_transf_to_idx'' b1 e1 && can_transf_to_idx'' b2 e2
-        | EIf e1 e2 e3 => can_transf_to_idx'' false e1 && can_transf_to_idx'' is_inv e2 && can_transf_to_idx'' is_inv e3
-        | ELet e1 x e2 => can_transf_to_idx'' false e1 && can_transf_to_idx'' is_inv e2
-        | EFlatmap e1 x e2 => can_transf_to_idx'' is_inv e1 && can_transf_to_idx'' is_inv e2
-        | EFold e1 e2 x y e3 => can_transf_to_idx'' false e1 && can_transf_to_idx'' false e2 && can_transf_to_idx'' false e3
-        | ERecord l => forallb (fun p => can_transf_to_idx'' false (snd p)) l
-        | EAccess e s => can_transf_to_idx'' false e
-        | EDict l => forallb (fun p => (can_transf_to_idx'' false (fst p) && can_transf_to_idx'' false (snd p))%bool) l
-        | EInsert d k v => can_transf_to_idx'' false d && can_transf_to_idx'' false k && can_transf_to_idx'' false v
-        | EDelete d k => can_transf_to_idx'' false d && can_transf_to_idx'' false k
-        | ELookup d k => can_transf_to_idx'' false d && can_transf_to_idx'' false k
-        | EOptMatch e e_none x e_some => can_transf_to_idx'' false e && can_transf_to_idx'' is_inv e_none && can_transf_to_idx'' is_inv e_some
-        | EDictFold d e0 k v acc e => can_transf_to_idx'' false d && can_transf_to_idx'' false e0 && can_transf_to_idx'' false e
-        | ESort l => can_transf_to_idx'' true l
-        | EFilter l x p => can_transf_to_idx'' is_inv l && can_transf_to_idx'' false p
-        | EJoin l1 l2 x1 x2 p r => can_transf_to_idx'' is_inv l1 && can_transf_to_idx'' is_inv l2 && can_transf_to_idx'' false p && can_transf_to_idx'' false r
-        | EProj l x r => can_transf_to_idx'' is_inv l && can_transf_to_idx'' false r
-        end.
-
-      Fixpoint can_transf_to_idx' (c : command) : bool :=
-        match c with
-        | CSkip => true
-        | CSeq c1 c2 => can_transf_to_idx' c1 && can_transf_to_idx' c2
-        | CLet e x c => can_transf_to_idx'' false e && can_transf_to_idx' c
-        | CLetMut e x c => negb (String.eqb x tbl) && can_transf_to_idx'' false e && can_transf_to_idx' c
-        | CAssign x e => can_transf_to_idx'' false e
-        | CIf e c1 c2 => can_transf_to_idx'' false e && can_transf_to_idx' c1 && can_transf_to_idx' c2
-        | CForeach e x c => can_transf_to_idx'' false e && can_transf_to_idx' c
-        end.
-
-      Definition can_transf_to_idx (c : command) : bool :=
-        match c with
-        | CLetMut (EAtom (ANil (Some (TRecord rt)))) x c =>
-            String.eqb x tbl &&
-              inb String.eqb attr (List.map fst rt) &&
-              can_transf_to_idx' c
-        | _ => false
-        end.
-    End __.
-
-    Definition transf_to_idx' (tbl attr : string) (c : command) : command :=
-      fold_command (list_write_to_idx_write tbl attr) (idx_read_to_list_read tbl) c.
-
-    Definition transf_to_idx (tbl attr : string) (c : command) : command :=
-      match c with
-      | CLetMut (EAtom (ANil _)) tbl' c =>
-          CLetMut (EDict nil) tbl (* Rely on can_transf_to_idx to check tbl' = tbl *)
-            (transf_to_idx' tbl attr c)
-      | _ => c
-      end.
-
-    Create HintDb fiat2_hints.
-
-    Local Ltac invert_type_wf :=
-      lazymatch goal with
-      | H: type_wf (TList ?t) |- type_wf ?t => inversion H; clear H; subst
-      | H: type_wf (TOption ?t) |- type_wf ?t => inversion H; clear H; subst
-      | H: type_wf (TDict ?t _) |- type_wf ?t => inversion H; clear H; subst
-      | H: type_wf (TDict _ ?t) |- type_wf ?t => inversion H; clear H; subst
-      | H: type_wf (TRecord ?tl) |- Forall type_wf (List.map snd ?tl) => inversion H; clear H; subst
-      end.
-
-    Lemma invert_TList_wf: forall t, type_wf (TList t) -> type_wf t.
-    Proof.
-      intros. invert_type_wf; auto.
-    Qed.
-
-    Lemma invert_TOption_wf: forall t, type_wf (TOption t) -> type_wf t.
-    Proof.
-      intros. invert_type_wf; auto.
-    Qed.
-
-    Lemma invert_TDict_wf_l: forall kt vt, type_wf (TDict kt vt) -> type_wf kt.
-    Proof.
-      intros. invert_type_wf; auto.
-    Qed.
-
-    Lemma invert_TDict_wf_r: forall kt vt, type_wf (TDict kt vt) -> type_wf vt.
-    Proof.
-      intros. invert_type_wf; auto.
-    Qed.
-
-    Lemma invert_TRecord_wf: forall tl, type_wf (TRecord tl) -> Forall type_wf (List.map snd tl).
-    Proof.
-      intros. invert_type_wf; auto.
-    Qed.
-
-    Hint Resolve invert_TList_wf : fiat2_hints.
-    Hint Resolve invert_TOption_wf : fiat2_hints.
-    Hint Resolve invert_TDict_wf_l : fiat2_hints.
-    Hint Resolve invert_TDict_wf_r : fiat2_hints.
-    Hint Resolve invert_TRecord_wf : fiat2_hints.
-(*
-    Local Ltac apply_type_of__type_wf :=
-      lazymatch goal with
-      | H: type_of _ _ _ ?t |- type_wf ?t =>
-          let H' := fresh "H'" in
-          apply type_of__type_wf in H as H'
-      | H: type_of _ _ _ (TList ?t) |- type_wf ?t =>
-          let H' := fresh "H'" in
-          apply type_of__type_wf in H as H'
-      | H:  type_of _ _ _ (TOption ?t) |- type_wf ?t =>
-          let H' := fresh "H'" in
-          apply type_of__type_wf in H as H'
-      | H:  type_of _ _ _ (TDict ?t _) |- type_wf ?t =>
-          let H' := fresh "H'" in
-          apply type_of__type_wf in H as H'
-      | H:  type_of _ _ _ (TDict _ ?t) |- type_wf ?t =>
-          let H' := fresh "H'" in
-          apply type_of__type_wf in H as H'
-      | H:  type_of _ _ _ (TRecord ?tl) |- context[?tl] =>
-          let H' := fresh "H'" in
-          apply type_of__type_wf in H as H'
-      end.
-
-    Lemma type_of_TList__type_wf : forall Gstore Genv e t,
-        tenv_wf Gstore -> tenv_wf Genv ->
-        type_of Gstore Genv e (TList t) -> type_wf t.
-    Proof.
-      intros; apply_type_of__type_wf; auto with fiat2_hints.
-    Qed.
-
-    Lemma type_of_TOption__type_wf : forall Gstore Genv e t,
-        tenv_wf Gstore -> tenv_wf Genv ->
-        type_of Gstore Genv e (TOption t) -> type_wf t.
-    Proof.
-      intros; apply_type_of__type_wf; auto with fiat2_hints.
-    Qed.
-
-    Lemma type_of_TDict__type_wf_l : forall Gstore Genv e kt vt,
-        tenv_wf Gstore -> tenv_wf Genv ->
-        type_of Gstore Genv e (TDict kt vt) -> type_wf kt.
-    Proof.
-      intros; apply_type_of__type_wf; eauto with fiat2_hints.
-    Qed.
-
-    Lemma type_of_TDict__type_wf_r : forall Gstore Genv e kt vt,
-        tenv_wf Gstore -> tenv_wf Genv ->
-        type_of Gstore Genv e (TDict kt vt) -> type_wf vt.
-    Proof.
-      intros; apply_type_of__type_wf; eauto with fiat2_hints.
-    Qed.
-
-    Lemma type_of_TRecord__type_wf : forall Gstore Genv e tl,
-        tenv_wf Gstore -> tenv_wf Genv ->
-        type_of Gstore Genv e (TRecord tl) -> Forall type_wf (List.map snd tl).
-    Proof.
-      intros. apply_type_of__type_wf. auto with fiat2_hints.
-    Qed.
-*)
-    Hint Resolve type_of__type_wf : fiat2_hints.
-
-
-    Local Ltac destruct_match :=
-      match goal with
-      | H: context[match ?x with _ => _ end] |- _ =>
-          let E := fresh "E" in
-          destruct x eqn:E
-      end.
-
-    Lemma locals_eq_update : forall (l l' : locals) x v,
-        (forall y, x <> y -> map.get l y = map.get l' y) ->
-        map.update l x v = map.update l' x v.
-    Proof.
-      intros * H. apply map.map_ext. intro y. destruct (String.eqb x y) eqn:E.
-      - rewrite eqb_eq in E; subst. repeat rewrite Properties.map.get_update_same; trivial.
-      - rewrite eqb_neq in E. repeat rewrite Properties.map.get_update_diff; auto.
-    Qed.
+    Definition tenv_equiv_at (x attr : string) (rt : list (string * type)) (Gstore : tenv) :=
+      map.put Gstore x (index_type (get_attr_type rt attr) rt).
 
     Definition locals_eq_except (x : string) (l l' : locals) :=
       forall y, x <> y -> map.get l y = map.get l' y.
@@ -623,30 +543,15 @@ Section WithWord.
       | _ => False
       end.
 
-    Definition tenv_eq_except (x : string) (G G' : tenv) :=
-      forall y, x <> y -> map.get G y = map.get G' y.
+    Lemma locals_eq_update : forall (l l' : locals) x v,
+        (forall y, x <> y -> map.get l y = map.get l' y) ->
+        map.update l x v = map.update l' x v.
+    Proof.
+      intros * H. apply map.map_ext. intro y. destruct (String.eqb x y) eqn:E.
+      - rewrite eqb_eq in E; subst. repeat rewrite Properties.map.get_update_same; trivial.
+      - rewrite eqb_neq in E. repeat rewrite Properties.map.get_update_diff; auto.
+    Qed.
 
-    Definition tenv_equiv_idx_list_at (x attr : string) (G G' : tenv) :=
-      match map.get G x with
-      | Some (TDict kt vt) =>
-          match map.get G' x with
-          | Some (TList (TRecord rt)) => In attr (List.map fst rt) /\ kt = get_attr_type rt attr /\ vt = TList (TRecord rt)
-          | _ => False
-          end
-      | _ => False
-      end.
-
-    Local Ltac get_update_same_diff x y :=
-      let E := fresh "E" in
-      destruct (String.eqb x y) eqn:E;
-      [ rewrite eqb_eq in E; subst; repeat rewrite Properties.map.get_update_same
-      | rewrite eqb_neq in E; repeat rewrite Properties.map.get_update_diff ]; auto.
-
-    Local Ltac get_put_same_diff x y :=
-      let E := fresh "E" in
-      destruct (String.eqb x y) eqn:E;
-      [ rewrite eqb_eq in E; subst; repeat rewrite map.get_put_same
-      | rewrite eqb_neq in E; repeat rewrite map.get_put_diff ]; auto.
 
     Lemma locals_eq_except_update : forall l l' tbl x v,
         locals_eq_except tbl l l' -> locals_eq_except tbl (map.update l x v) (map.update l' x v).
@@ -702,36 +607,11 @@ Section WithWord.
     Hint Resolve get_attr_type_ty_wf : fiat2_hints.
     Hint Resolve tenv_wf_step : fiat2_hints.
     Hint Resolve locals_wf_step : fiat2_hints.
-
-    Definition tenv_equiv_at (x attr : string) (rt : list (string * type)) (Gstore : tenv) :=
-      map.put Gstore x (TDict (get_attr_type rt attr) (TList (TRecord rt))).
-
-    Lemma locals_equiv_locals_wf : forall x rt attr Gstore' store' store,
-        locals_wf Gstore' store' ->
-        tenv_wf Gstore' ->
-        locals_equiv_idx_list_at x attr store store' ->
-        locals_eq_except x store store' ->
-        map.get Gstore' x = Some (TList (TRecord rt)) ->
-        In attr (List.map fst rt) ->
-        locals_wf (tenv_equiv_at x attr rt Gstore') store.
-    Proof.
-      intros * H_wf H_Gstr' H_equiv H_except H_x H_in. unfold tenv_equiv_at.
-      unfold locals_wf; intros y t. get_put_same_diff x y.
-      - intro H_t; injection H_t as H_t; subst.
-        unfold locals_equiv_idx_list_at in H_equiv. repeat destruct_match; intuition.
-        apply H_wf in H_x as H'. rewrite E1 in H'. subst.
-        assert (interp_expr store' map.empty (ELoc y) = VList l0). { simpl; unfold get_local. rewrite E1; auto. }
-        assert (interp_expr store' map.empty (list_to_idx attr (ELoc y)) = VDict (gallina_list_to_idx attr l0)).
-        { eapply fiat2_gallina_list_to_idx with (Genv:=map.empty); eauto.
-          1: constructor; auto.
-          1,2: unfold tenv_wf, locals_wf; intros; repeat rewrite map.get_empty in *; discriminate. }
-        assert (type_of Gstore' map.empty (ELoc y) (TList (TRecord rt))). { constructor; auto. }
-        eapply list_to_idx_preserve_ty in H1; eauto.
-        1: eapply type_sound with (env:=map.empty) in H1; eauto.
-        2-4: unfold tenv_wf, locals_wf; intros; repeat rewrite map.get_empty in *; discriminate.
-        rewrite H0 in H1. auto.
-      - intro H_y. apply H_wf in H_y. destruct_match; intuition. rewrite H_except; auto. rewrite E0; auto.
-    Qed.
+    Hint Resolve locals_eq_except_put : fiat2_hints.
+    Hint Resolve locals_equiv_idx_list_at_put : fiat2_hints.
+    Hint Resolve locals_eq_except_put0 : fiat2_hints.
+    Hint Resolve locals_equiv_idx_list_at_put0 : fiat2_hints.
+    Hint Resolve type_sound : fiat2_hints.
 
     Lemma tenv_equiv_at_wf : forall tbl attr rt Gstore,
         tenv_wf Gstore -> map.get Gstore tbl = Some (TList (TRecord rt)) ->
@@ -739,484 +619,716 @@ Section WithWord.
     Proof.
       intros * H_Gstr H_tbl_ty. apply tenv_wf_step; auto. constructor.
       all: apply H_Gstr in H_tbl_ty; auto with fiat2_hints.
+      repeat (constructor; simpl; intuition). congruence.
     Qed.
 
     Hint Resolve tenv_equiv_at_wf : fiat2_hints.
-    Hint Resolve locals_equiv_locals_wf : fiat2_hints.
-    Hint Resolve locals_eq_except_put : fiat2_hints.
-    Hint Resolve locals_equiv_idx_list_at_put : fiat2_hints.
-    Hint Resolve locals_eq_except_put0 : fiat2_hints.
-    Hint Resolve locals_equiv_idx_list_at_put0 : fiat2_hints.
-    Hint Resolve type_sound : fiat2_hints.
 
-    Lemma transf_read_preserve_ty : forall Gstore Genv x attr rt e t,
-        tenv_wf Gstore -> tenv_wf Genv ->
-        map.get Gstore x = Some (TList (TRecord rt)) -> type_of Gstore Genv e t ->
-        type_of (tenv_equiv_at x attr rt Gstore) Genv (fold_expr (idx_read_to_list_read x) e) t.
-    Proof.
-      intros * H_Gstr H_Genv H_x H_ty. unfold tenv_equiv_at.
-      generalize dependent Genv. generalize dependent t.
-      induction e using expr_IH; simpl; intros.
-      all: inversion H_ty; subst.
-      all: try now (econstructor; eauto).
-      - get_put_same_diff x x0.
-        + rewrite H0 in H_x; injection H_x as H_x; subst.
-          eapply idx_to_list_preserve_ty; eauto with fiat2_hints.
-          constructor. rewrite map.get_put_same. eauto.
-        + constructor. rewrite map.get_put_diff; congruence.
-      - econstructor; eauto. apply IHe2; eauto with fiat2_hints.
-      - econstructor; eauto. apply IHe2; auto. eauto with fiat2_hints.
-      - econstructor; eauto. apply IHe3; auto. repeat apply tenv_wf_step; eauto with fiat2_hints.
-      - econstructor; eauto.
-        + rewrite fst_map_fst; auto.
-        + clear H_ty H1 H3 H4 H5. generalize dependent tl. induction l; simpl; intros.
-          1: inversion H2; constructor.
-          destruct tl; simpl in *; inversion H2; subst. constructor; inversion H; subst.
-          1: destruct a; simpl in *; apply H3; auto.
-          apply IHl; auto; injection H1; intros; auto.
-      - econstructor; eauto. clear H_ty. induction H3; intuition. constructor; inversion H; subst.
-        1: destruct x0; simpl in *; split; apply H7; auto.
-        1: apply IHForall; auto.
-      - econstructor; eauto. apply IHe3; eauto with fiat2_hints.
-      - econstructor; eauto. apply IHe3; auto. repeat apply tenv_wf_step; eauto with fiat2_hints.
-      - constructor; auto. apply IHe2; eauto with fiat2_hints.
-      - econstructor; eauto.
-        1: apply IHe3; auto. 2: apply IHe4; eauto with fiat2_hints.
-        all: repeat apply tenv_wf_step; eauto with fiat2_hints.
-      - econstructor; eauto. apply IHe2; eauto with fiat2_hints.
-    Qed.
+    Section list_idx.
+      Context (tup acc x k v : string).
 
-    Local Ltac invert_unop_binop_atom_ty :=
-      lazymatch goal with
-      | H: type_of_unop _ _ _ |- _ => inversion H; subst
-      | H: type_of_binop _ _ _ _ |- _ => inversion H; subst
-      | H: type_of_atom _ _ |- _ => inversion H; subst
-      end.
+      (* Materialize tbl (expected to be a list of records) into an index over attr *)
+      Definition list_to_idx (attr : string) (tbl : expr) : expr :=
+        let k := EAccess (EVar tup) attr in
+        EFold tbl (EDict nil) tup acc
+          (EInsert (EVar acc) k
+             (EOptMatch (ELookup (EVar acc) k)
+                (epair enil (EVar tup))
+                x (cons_to_fst (EVar tup) (EVar x)))).
 
-    Local Ltac apply_transf_read_write_sound''_IH Gstore' :=
-      lazymatch goal with
-      | H: context[type_of _ _ ?e _ -> _],
-          H_can: can_transf_to_idx'' _ false ?e = true,
-            H_equiv: locals_equiv_idx_list_at _ _ _ _ |- _ =>
-          let IH := fresh "IH" in
-          let IHL := fresh "IHL" in
-          let IH' := fresh "IH'" in
-          eapply H with (Gstore':=Gstore') in H_equiv as IH; eauto; clear H;
-          try (destruct IH as [IHL _]; apply IHL in H_can as IH')
-      | H: context[type_of _ _ ?e _ -> _],
-          H_can: can_transf_to_idx'' _ true ?e = true,
-            H_equiv: locals_equiv_idx_list_at _ _ _ _ |- _ =>
-          let IH := fresh "IH" in
-          let IHR := fresh "IHR" in
-          let IH' := fresh "IH'" in
-          eapply H with (Gstore':=Gstore') in H_equiv as IH; eauto; clear H;
-          try (destruct IH as [_ IHR]; apply IHR in H_can as IH')
-      end.
+      (* Inverse of tbl_to_idx, expecting idx to be a dict
+   Require the index keys in idx to match the attr values in the records *)
+      Definition idx_to_list (idx : expr) : expr :=
+        EDictFold idx enil k v acc
+          (EBinop OConcat (ofst (EVar v))
+             (econs (osnd (EVar v)) (EVar acc))).
 
-    Local Ltac apply_Forall_In :=
-      lazymatch goal with
-      | H1: Forall _ ?l, H2: In _ ?l |- _ => eapply List.Forall_In in H1; eauto
-      end.
-
-    Local Ltac rewrite_expr_value :=
-      lazymatch goal with
-      | E: VList _ = ?e |- context[?e] => rewrite <- E
-      | E: VList _ = ?e, H: context[?e] |- _ => rewrite <- E in H
-      end.
-
-    Local Ltac apply_type_sound e :=
+      Lemma fiat2_gallina_list_to_idx : forall (Gstore Genv : tenv) (store env : locals) tbl attr l rt,
+          is_NoDup [tup; acc; x] ->
+          tenv_wf Gstore -> tenv_wf Genv ->
+          type_of Gstore Genv tbl (TList (TRecord rt)) ->
+          In attr (List.map fst rt) ->
+          locals_wf Gstore store -> locals_wf Genv env ->
+          interp_expr store env tbl = VList l ->
+          interp_expr store env (list_to_idx attr tbl) = VDict (gallina_list_to_idx attr l).
+      Proof.
+        intros * vars_distinct H_Gstr H_Genv H_ty H_in H_str H_env H_tbl_v.
+        simpl. rewrite H_tbl_v.
+        eapply type_sound in H_ty; eauto. rewrite H_tbl_v in H_ty. inversion H_ty; subst.
+        erewrite In_fold_right_ext with
+          (P := fun a => match a with VDict _ => True | _ => False end)
+          (g := fun v1 v2 => match v1, v2 with
+                             | VRecord l1, VDict l0 =>
+                                 VDict
+                                   (dict_insert (record_proj attr l1)
+                                      match dict_lookup (record_proj attr l1) l0 with
+                                      | Some v0 =>
+                                          VRecord
+                                            [("0",
+                                               match
+                                                 match v0 with
+                                                 | VRecord l2 => record_proj "0" l2
+                                                 | _ => VUnit
+                                                 end
+                                               with
+                                               | VList l2 => VList (VRecord l1 :: l2)
+                                               | _ => VUnit
+                                               end);
+                                             ("1",
+                                               match v0 with
+                                               | VRecord l2 => record_proj "1" l2
+                                               | _ => VUnit
+                                               end)]
+                                      | None => VRecord (record_sort [("0", VList []); ("1", VRecord l1)])
+                                      end l0)
+                             | _, _ => VUnit
+                             end).
+        3:{ intros a b H_a H_in_b. destruct a; intuition.
+            all: unfold get_local; repeat rewrite_map_get_put_goal; auto.
+            apply_Forall_In. invert_type_of_value. do 2 f_equal.
             lazymatch goal with
-            | H: type_of _ _ e _ |- _ =>
-                let H' := fresh "H'" in
-                eapply type_sound in H as H'; eauto; try inversion H'; subst; auto
-            end.
+            | |- context[dict_lookup ?a ?b] => destruct (dict_lookup a b)
+            end; simpl; auto. f_equal. repeat rewrite_map_get_put_goal; auto. }
+        2: trivial.
+        1:{ clear H_tbl_v H_ty. induction l; simpl; auto. invert_Forall; subst. rewrite IHl; auto. clear IHl.
+            invert_type_of_value. do 2 f_equal. simpl.
+            lazymatch goal with
+            | |- context[dict_lookup ?a ?b] => destruct (dict_lookup a b)
+            end; simpl; auto. f_equal. destruct v0; auto. }
+      Qed.
 
-    Local Ltac rewrite_interp_fold_expr :=
-      lazymatch goal with
-      | H: interp_expr _ _ (fold_expr _ ?e) = _ |- context[?e] =>
-          rewrite H; clear H
-      end.
+      Lemma fiat2_gallina_idx_to_list : forall (Gstore Genv : tenv) (store env : locals) idx l kt rt,
+          is_NoDup [acc; v] ->
+          tenv_wf Gstore -> tenv_wf Genv ->
+          type_of Gstore Genv idx (index_type kt rt) ->
+          locals_wf Gstore store -> locals_wf Genv env ->
+          interp_expr store env idx = VDict l ->
+          interp_expr store env (idx_to_list idx) = VList (gallina_idx_to_list l).
+      Proof.
+        intros * vars_distinct H_Gstr H_Genv H_ty H_str H_env H_idx_v.
+        eapply type_sound in H_ty; eauto. rewrite H_idx_v in H_ty; inversion H_ty; subst.
+        simpl. rewrite H_idx_v.
+        erewrite In_fold_right_ext with
+          (P := fun v => match v with VList _ => True | _ => False end).
+        3:{ intros a b H_a H_in_b. unfold get_local.
+            repeat rewrite_map_get_put_goal.
+            apply_Forall_In. intuition. invert_type_of_value. destruct a; intuition.
+            inversion H9; subst. destruct x0; intuition. unfold record_proj.
+            simpl in *; subst. invert_type_of_value; auto. }
+        2: trivial.
+        1:{ clear H_idx_v H_ty H5 H6. induction l; simpl; auto. invert_Forall.
+            rewrite IHl; auto. clear IHl. intuition. invert_type_of_value.
+            invert_Forall2; subst. destruct x0; intuition; simpl in *. subst.
+            invert_type_of_value; auto. }
+      Qed.
 
-    Lemma In_map_ext : forall A B (f g : A -> B) l, (forall x, In x l -> f x = g x) -> List.map f l = List.map g l.
-    Proof.
-      intros * H. induction l; simpl; auto.
-      f_equal; [ apply H | apply IHl ]; intuition.
-    Qed.
+      Lemma fiat2_gallina_list_to_idx_to_list : forall (Gstore Genv : tenv) (store env : locals) l attr tbl rt,
+          is_NoDup [tup; acc; x; v] ->
+          tenv_wf Gstore -> tenv_wf Genv ->
+          type_of Gstore Genv tbl (TList (TRecord rt)) ->
+          In attr (List.map fst rt) ->
+          locals_wf Gstore store -> locals_wf Genv env ->
+          interp_expr store env tbl = VList l ->
+          interp_expr store env (idx_to_list (list_to_idx attr tbl)) =
+            VList (gallina_idx_to_list (gallina_list_to_idx attr l)).
+      Proof.
+        intros * vars_distinct H_Gstr H_Genv H_ty H_in H_str H_env H_tbl_v.
+        apply In_access_record in H_in as Ht. destruct Ht as [t Ht].
+        eapply fiat2_gallina_idx_to_list with (Gstore:=Gstore) (kt:=t); eauto.
+        1: simpl in *; intuition.
+        2:{ eapply fiat2_gallina_list_to_idx with (Gstore:=Gstore); eauto. simpl in *; intuition. }
+        apply type_of__type_wf in H_ty as H_wf; auto. inversion H_wf; subst.
+        repeat (try econstructor; try erewrite map.get_put_same; try erewrite map.get_put_diff; eauto).
+        1: eapply access_record_type_wf; eauto.
+        1, 5, 8: simpl; try rewrite <- eqb_eq; intuition.
+        all: simpl in *; intuition.
+      Qed.
 
-    Lemma Permutation_filter : forall A (l l' : list A), Permutation l l' -> forall f, Permutation (filter f l) (filter f l').
-    Proof.
-      induction l; intros.
-      - apply Permutation_nil in H. subst. auto.
-      - apply Permutation_sym in H as H'. apply Permutation_vs_cons_inv in H'.
-        repeat lazymatch goal with H: exists _, _ |- _ => destruct H end.
-        subst. rewrite filter_app. simpl; destruct (f a).
-        1: apply Permutation_cons_app.
-        all: rewrite <- filter_app.
-        all: apply Permutation_cons_app_inv in H; auto.
-    Qed.
+      Lemma list_to_idx_preserve_ty : forall Gstore Genv tbl rt attr,
+          is_NoDup [tup; acc; x] ->
+          tenv_wf Gstore -> tenv_wf Genv ->
+          In attr (List.map fst rt) ->
+          type_of Gstore Genv tbl (TList (TRecord rt)) ->
+          type_of Gstore Genv (list_to_idx attr tbl) (TDict (get_attr_type rt attr) (TRecord [("0", (TList (TRecord rt))); ("1", TRecord rt)])).
+      Proof.
+        intros * vars_distinct H_Gstr H_Genv H_in H_ty.
+        eapply type_of__type_wf in H_ty as H_wf; auto. inversion H_wf; subst.
+        inversion H0; subst.
+        repeat (econstructor; eauto; repeat rewrite_map_get_put_goal).
+        all: try rewrite <- inb_false_iff; auto.
+        all: unfold get_attr_type; apply In_access_record in H_in as [t Ht]; try rewrite Ht; auto.
+        apply access_record_sound in Ht; apply in_map with (f:=snd) in Ht; apply_Forall_In.
+      Qed.
 
-    Lemma Permutation_flat_map : forall A B (f g : A -> list B),
-                   forall l l', (forall x, In x l -> Permutation (f x) (g x)) ->
-                                Permutation l l' ->
-                                Permutation (flat_map f l) (flat_map g l').
-    Proof.
-      intros * H_fg. generalize dependent l'. induction l; simpl; intros l' H.
-      - apply Permutation_nil in H; subst; auto.
-      - apply Permutation_sym in H as H'. apply Permutation_vs_cons_inv in H'.
-        repeat lazymatch goal with H: exists _, _ |- _ => destruct H end. subst.
-        rewrite flat_map_app. simpl. pose proof H_fg a as H_a.
-        assert (H_a_in: In a (a :: l)). { intuition. } apply H_a in H_a_in as H_p.
-        destruct (f a) eqn:E.
-        + simpl. apply Permutation_nil in H_p.
-          rewrite H_p; simpl. rewrite <- flat_map_app.
-          apply Permutation_cons_app_inv in H. intuition.
-        + eapply perm_trans. 2: apply Permutation_app_swap_app.
-          apply Permutation_app; auto. rewrite <- flat_map_app. apply IHl.
-          2: apply Permutation_cons_app_inv in H.
-          all: intuition.
-    Qed.
+      Lemma idx_to_list_preserve_ty : forall Gstore Genv idx kt t,
+          is_NoDup [acc; v] ->
+          tenv_wf Gstore -> tenv_wf Genv ->
+          type_of Gstore Genv idx (TDict kt (TRecord [("0", TList t); ("1", t)])) ->
+          type_of Gstore Genv (idx_to_list idx) (TList t).
+      Proof.
+        intros * vars_distinct H_Gstr H_Genv H_ty. eapply type_of__type_wf in H_ty as H_wf; auto.
+        inversion H_wf; subst. inversion H2; subst; simpl in *.
+        repeat (econstructor; eauto; repeat rewrite_map_get_put_goal).
+        all: try lazymatch goal with
+               | |- type_wf _ => idtac; eapply List.Forall_In; eauto; intuition
+               end.
+      Qed.
 
-    Local Ltac apply_transf_read_preserve_ty e attr :=
-      lazymatch goal with
-      | H: type_of _ _ e _ |- _ =>
-          let H_transf_ty := fresh "H_transf_ty" in
-          eapply transf_read_preserve_ty with (attr:=attr) in H as H_transf_ty; eauto with fiat2_hints;
-          apply_type_sound e;
-          eapply type_sound in H_transf_ty; eauto with fiat2_hints;
-          inversion H_transf_ty; subst
-      end.
+      Lemma gallina_list_to_idx_shape : forall l attr rt,
+          Forall (fun v => type_of_value v (TRecord rt)) l ->
+          In attr (List.map fst rt) ->
+          Forall has_index_entry_shape (gallina_list_to_idx attr l).
+      Proof.
+        intros * H_ty H_in. induction H_ty; simpl; auto.
+        invert_type_of_value.
+        specialize (dict_insert_incl (width:=width)) as H_ins.
+        eapply incl_Forall; eauto.
+        constructor; intuition. simpl. unfold has_index_entry_shape in *.
+        lazymatch goal with
+        | |- context[dict_lookup ?k ?d] => destruct (dict_lookup k d) eqn:E
+        end; simpl; intuition.
+        eapply Forall_dict_lookup in IHH_ty; simpl in IHH_ty; eauto.
+        destruct v0; intuition. destruct (record_proj "0" l1); intuition.
+      Qed.
 
-    Lemma imp_pre_true : forall A B, A -> (A -> B) -> A /\ B.
-    Proof. intuition. Qed.
+      Lemma gallina_list_to_idx_SSorted : forall l attr rt,
+          Forall (fun v => type_of_value v (TRecord rt)) l ->
+          In attr (List.map fst rt) ->
+          StronglySorted dict_entry_leb (gallina_list_to_idx attr l).
+      Proof.
+        intros; induction l; simpl; try constructor.
+        inversion H; subst. inversion H3; subst.
+        apply dict_insert_preserve_SSorted; auto.
+      Qed.
 
-    Lemma transf_read_write_sound'' : forall tbl attr rt e Gstore' Genv t store store' env,
-        type_of Gstore' Genv e t ->
-        tenv_wf Gstore' -> tenv_wf Genv ->
-        map.get Gstore' tbl = Some (TList (TRecord rt)) -> In attr (List.map fst rt) ->
-        locals_wf Gstore' store' -> locals_wf Genv env ->
-        locals_eq_except tbl store store' ->
-        locals_equiv_idx_list_at tbl attr store store' ->
-        (can_transf_to_idx'' tbl false e -> interp_expr store env (fold_expr (idx_read_to_list_read tbl) e) = interp_expr store' env e) /\
-          (can_transf_to_idx'' tbl true e ->
-           match t with
-           | TList t =>
-               match interp_expr store env (fold_expr (idx_read_to_list_read tbl) e) with
-               | VList l => match interp_expr store' env e with
-                            | VList l' => Permutation l l'
-                            | _ => False
-                            end
-               | _ => False
-               end
-           | _ => interp_expr store env (fold_expr (idx_read_to_list_read tbl) e) = interp_expr store' env e
-           end).
-    Proof.
-      induction e using expr_IH; cbn; intros * H_ty H_Gstr' H_Genv H_tbl_ty H_in H_str' H_env H_except H_equiv; auto.
-      - (* EVar *)
-        split; intros; auto. apply_type_sound (EVar x).
-      - (* ELoc *)
-        split; intros.
-        all: unfold is_true in *; rewrite Bool.orb_true_iff in H.
-        + destruct (String.eqb x tbl) eqn:E; intuition; try discriminate.
-          rewrite eqb_sym; rewrite E; try discriminate. apply eqb_neq in E. simpl.
-          unfold get_local. rewrite H_except; auto.
-        +  clear H; destruct (String.eqb x tbl) eqn:E; rewrite eqb_sym; rewrite E.
-          * (* x = tbl *) rewrite eqb_eq in E; subst.
-            inversion H_ty; subst. rewrite H0 in H_tbl_ty. injection H_tbl_ty; intros; subst.
-            apply_type_sound (ELoc tbl).
-            erewrite fiat2_gallina_idx_to_list with (Gstore:=tenv_equiv_at tbl attr rt Gstore'); simpl; eauto with fiat2_hints.
-            1: eapply gallina_list_to_idx_to_list; eauto.
-            1:{ constructor. unfold tenv_equiv_at. rewrite map.get_put_same. eauto. }
-            1:{ unfold get_local. unfold locals_equiv_idx_list_at in H_equiv; repeat destruct_match; intuition.
-                subst. unfold get_local in *. rewrite E1 in H. injection H; congruence. }
-          * (* x <> tbl *) rewrite eqb_neq in E. destruct t; simpl.
-            all: unfold get_local; rewrite H_except; auto.
-            apply_type_sound (ELoc x). unfold get_local in *.
-            rewrite_expr_value. intuition.
-      - (* EAtom *)
-        split; intro H_can; destruct t; auto. inversion H_ty; subst. invert_unop_binop_atom_ty.
-        all: simpl; intuition.
-      - (* EUnop *)
-        inversion H_ty; subst. split; intro H_can; destruct o; simpl in *.
-        all: invert_unop_binop_atom_ty; unfold is_true in H_can.
-        all: apply_transf_read_write_sound''_IH Gstore'; try rewrite IH'; auto.
-        (* OLength *)
-        all: apply_transf_read_preserve_ty e attr.
-        all: repeat rewrite_expr_value.
-        all: erewrite Permutation_length; eauto.
-      - (* EBinop *)
-        inversion H_ty; subst. split; intro H_can; destruct o; simpl in *.
-        all: invert_unop_binop_atom_ty; unfold is_true in H_can; repeat rewrite Bool.andb_true_iff in H_can; intuition.
-        all: repeat apply_transf_read_write_sound''_IH Gstore'; try congruence.
-        all: try now (repeat rewrite_interp_fold_expr; auto).
-        1,2,4,5: (* OConcat, ORepeat, ORange, OWRange *)
-          repeat rewrite_interp_fold_expr; auto;
-        apply_type_sound e1; apply_type_sound e2; auto.
-        (* OCons *)
-        rewrite_interp_fold_expr.
-        eapply locals_equiv_locals_wf in H_equiv as H_wf; eauto.
-        apply_transf_read_preserve_ty e2 attr.
-        apply perm_skip. repeat rewrite_expr_value; auto.
-      - (* EIf *)
-        inversion H_ty; subst. split; intro H_can.
-        all: unfold is_true in H_can; repeat rewrite Bool.andb_true_iff in H_can; intuition.
-        all: repeat apply_transf_read_write_sound''_IH Gstore';
-          repeat rewrite_interp_fold_expr; auto.
-        apply_type_sound e1. destruct b; auto.
-      - (* ELet *)
-        inversion H_ty; subst. split; intro H_can.
-        all: unfold is_true in H_can; repeat rewrite Bool.andb_true_iff in H_can; intuition.
-        all: repeat apply_transf_read_write_sound''_IH Gstore';
-          repeat rewrite_interp_fold_expr; eauto with fiat2_hints.
-      - (* EFlatmap *)
-        inversion H_ty; subst. split; intro H_can.
-        all: unfold is_true in H_can; repeat rewrite Bool.andb_true_iff in H_can; intuition.
-        all: revert IHe2; apply_transf_read_write_sound''_IH Gstore'; intros.
-        + rewrite_interp_fold_expr; auto. apply_type_sound e1. f_equal.
-          apply In_flat_map_ext. intros a H_a_in. apply_transf_read_write_sound''_IH Gstore'; try rewrite_interp_fold_expr; eauto with fiat2_hints.
-          1: apply locals_wf_step; auto; apply_Forall_In.
-        + eapply locals_equiv_locals_wf in H_equiv as H_wf; eauto.
-          apply_transf_read_preserve_ty e1 attr. repeat rewrite_expr_value.
-          apply Permutation_flat_map; auto.
-          intros v H_v_in. apply_Forall_In.
-          apply_transf_read_write_sound''_IH Gstore'; eauto with fiat2_hints.
-          1: apply_transf_read_preserve_ty e2 attr.
-          1: iter_hyps rewrite_hyp_l; auto.
-      - (* EFold *)
-        inversion H_ty; subst.
-        apply imp_pre_true.
-        1: intro H_can.
-        2: intros HA H_can; specialize (HA H_can).
-        all: unfold is_true in H_can; repeat rewrite Bool.andb_true_iff in H_can; intuition.
-        all: revert IHe3; repeat apply_transf_read_write_sound''_IH Gstore'; intros.
-        + repeat rewrite_interp_fold_expr. apply_type_sound e1.
-          eapply type_sound in H6 as H2'; eauto.
-          eapply In_fold_right_ext with (P:=fun a => type_of_value a t); auto.
-          intros * P H_b_in. intuition.
-          1:{ apply_transf_read_write_sound''_IH Gstore'; eauto.
-              1: repeat apply tenv_wf_step; eauto with fiat2_hints.
-              1: repeat apply locals_wf_step; eauto with fiat2_hints; apply_Forall_In. }
-          1:{ apply_transf_read_write_sound''_IH Gstore'; auto.
-              1: rewrite_interp_fold_expr; eapply type_sound; eauto.
-              1,3: repeat apply tenv_wf_step; eauto with fiat2_hints.
-              1,2: repeat apply locals_wf_step; eauto with fiat2_hints; apply_Forall_In. }
-        + rewrite HA. destruct t; auto.
-          apply_type_sound (EFold e1 e2 x y e3).
-      - (* ERecord *)
-        inversion H_ty; subst. split; intro H_can.
-        all: unfold is_true in H_can; repeat rewrite Bool.andb_true_iff in H_can; intuition.
-        all: do 2 f_equal; rewrite map_map.
-        all: apply In_map_ext; intros x H_x_in; apply_Forall_In;
-          rewrite forallb_forall in H_can; apply H_can in H_x_in as H_x.
-        all: apply in_map with (f:=snd) in H_x_in; pose proof (Forall2_In_Permuted _ _ _ _ _ _ H2 H_x_in).
-        all: do 3 destruct H0; intuition.
-        all: eapply H with (Gstore':=Gstore') in H_equiv as IH; eauto.
-        all: apply IH in H_x as IH'; destruct x; simpl in *; congruence.
-      - (* EAccess *)
-        inversion H_ty; subst. split; intro H_can.
-        all: unfold is_true in H_can; repeat rewrite Bool.andb_true_iff in H_can; intuition.
-        all: apply_transf_read_write_sound''_IH Gstore'; rewrite_interp_fold_expr; auto.
-        destruct t; auto. apply_type_sound (EAccess e s).
-      - (* EDict *)
-        inversion H_ty; subst. split; intro H_can.
-        all: unfold is_true in H_can.
-        all: do 3 f_equal; rewrite map_map; apply In_map_ext.
-        all: intros x H_x_in; destruct x; simpl in *.
-        all: repeat apply_Forall_In; rewrite forallb_forall in H_can; apply H_can in H_x_in as H_x.
-        all: repeat rewrite Bool.andb_true_iff in *; intuition; simpl in *.
-        all: repeat apply_transf_read_write_sound''_IH Gstore'.
-        all: rewrite IH', IH'0; auto.
-      - (* EInsert *)
-        inversion H_ty; subst. split; intro H_can.
-        all: unfold is_true in H_can; repeat rewrite Bool.andb_true_iff in H_can; intuition.
-        all: repeat apply_transf_read_write_sound''_IH Gstore'; repeat rewrite_interp_fold_expr; auto.
-      - (* EDelete *)
-        inversion H_ty; subst. split; intro H_can.
-        all: unfold is_true in H_can; repeat rewrite Bool.andb_true_iff in H_can; intuition.
-        all: repeat apply_transf_read_write_sound''_IH Gstore'; repeat rewrite_interp_fold_expr; auto.
-      - (* ELookup *)
-        inversion H_ty; subst. split; intro H_can.
-        all: unfold is_true in H_can; repeat rewrite Bool.andb_true_iff in H_can; intuition.
-        all: repeat apply_transf_read_write_sound''_IH Gstore'; repeat rewrite_interp_fold_expr; auto.
-      - (* EOptMatch *)
-        inversion H_ty; subst. split; intro H_can.
-        all: unfold is_true in H_can; repeat rewrite Bool.andb_true_iff in H_can; intuition.
-        all: revert IHe2 IHe3; apply_transf_read_write_sound''_IH Gstore'; intros.
-        all: rewrite_interp_fold_expr; apply_type_sound e1.
-        all: try now (revert IHe3; apply_transf_read_write_sound''_IH Gstore'; eauto).
-        all: revert IHe2; apply_transf_read_write_sound''_IH Gstore'; eauto with fiat2_hints.
-      - (* EDictFold *)
-        inversion H_ty; subst. apply imp_pre_true.
-        1: intro H_can.
-        2: intros HA H_can; specialize (HA H_can).
-        all: unfold is_true in H_can; repeat rewrite Bool.andb_true_iff in H_can; intuition.
-        all: revert IHe3; repeat apply_transf_read_write_sound''_IH Gstore'; intros.
-        + repeat rewrite_interp_fold_expr; apply_type_sound e1.
-          apply In_fold_right_ext with (P := fun a => type_of_value a t).
-          2:{ intros. apply_transf_read_write_sound''_IH Gstore'.
-              1: rewrite_interp_fold_expr.
-              2: repeat apply tenv_wf_step; eauto with fiat2_hints.
-              2: repeat apply locals_wf_step; auto; apply_Forall_In; intuition.
-              1: intuition. apply_type_sound e3; eauto with fiat2_hints.
-              1: repeat apply locals_wf_step; auto; apply_Forall_In; intuition. }
-          apply_type_sound e2; eauto.
-        + rewrite HA. destruct t; auto.
-          apply_type_sound (EDictFold e1 e2 k v acc e3).
-      - (* ESort *)
-        inversion H_ty; subst. split; intro H_can.
-        all: unfold is_true in H_can; repeat rewrite Bool.andb_true_iff in H_can; intuition.
-        all: apply_transf_read_write_sound''_IH Gstore'.
-        1:{ repeat destruct_match; intuition. f_equal. apply Permutation_SSorted_eq; auto using StronglySorted_value_sort.
-            pose proof Permuted_value_sort l. pose proof Permuted_value_sort l0.
-            eapply perm_trans. 2: eauto. apply Permutation_sym. eapply perm_trans. 2: eauto. apply Permutation_sym; auto. }
-        1:{ eapply locals_equiv_locals_wf in H_equiv as H_wf; eauto.
-            apply_transf_read_preserve_ty e attr. repeat rewrite_expr_value.
-            pose proof Permuted_value_sort l. pose proof Permuted_value_sort l0.
-            eapply perm_trans. 2: eauto. apply Permutation_sym. eapply perm_trans. 2: eauto. apply Permutation_sym; auto. }
-      - (* EFilter *)
-        inversion H_ty; subst. split; intro H_can.
-        all: unfold is_true in H_can; repeat rewrite Bool.andb_true_iff in H_can; intuition.
-        all: revert IHe2; apply_transf_read_write_sound''_IH Gstore'; intros.
-        + rewrite_interp_fold_expr. apply_type_sound e1. f_equal.
-          apply filter_ext_in; intros a H_a_in. apply_transf_read_write_sound''_IH Gstore'; eauto with fiat2_hints.
-          1: rewrite_interp_fold_expr; auto.
-          1: apply locals_wf_step; auto; apply_Forall_In.
-        + eapply locals_equiv_locals_wf in H_equiv as H_wf; eauto.
-          apply_transf_read_preserve_ty e1 attr. repeat rewrite_expr_value.
-          rewrite In_filter_ext with
-            (g:=fun v : value => match interp_expr store' (map.put env x v) e2 with
-                                 | VBool b => b
-                                 | _ => false
-                                 end).
-          2:{ intros a H_a_in. apply_transf_read_write_sound''_IH Gstore'; eauto with fiat2_hints.
-              1: rewrite_interp_fold_expr; auto.
-              1: apply locals_wf_step; auto; apply_Forall_In. }
-          apply Permutation_filter; auto.
-      - (* EJoin *)
-        inversion H_ty; subst. split; intro H_can.
-        all: unfold is_true in H_can; repeat rewrite Bool.andb_true_iff in H_can; intuition.
-        all: revert IHe3 IHe4; repeat apply_transf_read_write_sound''_IH Gstore'; intros.
-        + repeat rewrite_interp_fold_expr.
-          apply_type_sound e1. apply_type_sound e2. f_equal.
-          apply In_flat_map_ext; intros a H_a_in.
-          rewrite In_filter_ext with
-            (g:=fun v2 : value => match interp_expr store' (map.put (map.put env x a) y v2) e3 with
-                                  | VBool b => b
-                                  | _ => false
-                                  end).
-          1: apply In_map_ext; intros b H_b_in; revert IHe3; repeat apply_transf_read_write_sound''_IH Gstore'; auto.
-          1: repeat apply tenv_wf_step; eauto with fiat2_hints.
-          1: repeat apply locals_wf_step; eauto with fiat2_hints.
-          1,2: rewrite filter_In in H_b_in; intuition; repeat apply_Forall_In.
-          intros c H_c_in. revert IHe4; apply_transf_read_write_sound''_IH Gstore'; intros.
-          1: rewrite_interp_fold_expr; auto.
-          1: repeat apply tenv_wf_step; eauto with fiat2_hints.
-          1: repeat apply locals_wf_step; repeat apply_Forall_In.
-        + eapply locals_equiv_locals_wf in H_equiv as H_wf; eauto.
-          apply_transf_read_preserve_ty e1 attr.
-          apply_transf_read_preserve_ty e2 attr. repeat rewrite_expr_value.
-          apply Permutation_flat_map; auto. intros a H_a_in.
-          rewrite In_map_ext with (g:=fun v2 : value => interp_expr store' (map.put (map.put env x a) y v2) e4).
-          1: apply Permutation_map.
-          1: rewrite In_filter_ext with
-            (g:=fun v2 : value => match interp_expr store' (map.put (map.put env x a) y v2) e3 with
-                                  | VBool b => b
-                                  | _ => false
-                                  end).
-          1:{ apply Permutation_filter; auto. }
-          1:{ intros b H_b_in. revert IHe4; apply_transf_read_write_sound''_IH Gstore'; intros.
-              1: rewrite_interp_fold_expr; auto.
-              1: repeat apply tenv_wf_step; eauto with fiat2_hints.
-              1: repeat apply locals_wf_step; repeat apply_Forall_In. }
-          1:{ intros b H_b_in. revert IHe3; apply_transf_read_write_sound''_IH Gstore'; intros.
-              1: rewrite_interp_fold_expr; auto.
-              1: repeat apply tenv_wf_step; eauto with fiat2_hints.
-              1: repeat apply locals_wf_step; auto.
-              1,2: apply filter_In in H_b_in; intuition; repeat apply_Forall_In. }
-      - (* EProj *)
-        inversion H_ty; subst. split; intro H_can.
-        all: unfold is_true in H_can; repeat rewrite Bool.andb_true_iff in H_can; intuition.
-        all: revert IHe2; apply_transf_read_write_sound''_IH Gstore'; intros.
-        + rewrite_interp_fold_expr. apply_type_sound e1. f_equal. apply In_map_ext.
-          intros a H_a_in. apply_transf_read_write_sound''_IH Gstore'; eauto with fiat2_hints.
-          repeat apply locals_wf_step; apply_Forall_In.
-        + eapply locals_equiv_locals_wf in H_equiv as H_wf; eauto.
-          apply_transf_read_preserve_ty e1 attr.
-          rewrite In_map_ext with (g:=(fun v : value => interp_expr store' (map.put env x v) e2)).
-          2:{ intros a H_a_in. apply_transf_read_write_sound''_IH Gstore'; eauto with fiat2_hints.
-              repeat apply locals_wf_step; apply_Forall_In. }
-          repeat rewrite_expr_value. apply Permutation_map; auto.
-    Qed.
+      Lemma gallina_list_to_idx_Permutation : forall attr l rt,
+          Forall (fun v => type_of_value v (TRecord rt)) l ->
+          In attr (List.map fst rt) ->
+          Permutation (concat_VList_V (List.map snd (gallina_list_to_idx attr l))) l.
+      Proof.
+        intros * H_ty H_in. induction H_ty; simpl; auto.
+        invert_type_of_value. eapply perm_trans.
+        1:{ eapply dict_insert_lookup_Permutation.
+            - eapply gallina_list_to_idx_shape; eauto.
+            - eapply gallina_list_to_idx_SSorted; eauto. }
+        1: constructor; auto.
+      Qed.
 
-    Lemma transf_read_write_sound' : forall c Gstore' Genv rt store store' env tbl attr,
-        well_typed Gstore' Genv c ->
-        map.get Gstore' tbl = Some (TList (TRecord rt)) ->
-        In attr (List.map fst rt) ->
-        tenv_wf Gstore' -> tenv_wf Genv -> locals_wf Gstore' store' -> locals_wf Genv env ->
-        locals_eq_except tbl store store' ->
-        locals_equiv_idx_list_at tbl attr store store' ->
-        can_transf_to_idx' tbl c = true ->
-        (locals_eq_except tbl
-           (interp_command store env (transf_to_idx' tbl attr c))
-           (interp_command store' env c)) /\
-          (locals_equiv_idx_list_at tbl attr
+      Lemma gallina_idx_to_list__concat_VList_V : forall l,
+          Forall has_index_entry_shape l ->
+          gallina_idx_to_list l = concat_VList_V (List.map snd l).
+      Proof.
+        intros * H.
+        induction l; simpl; auto.
+        inversion H; subst.
+        destruct (snd a); intuition. rewrite H0. reflexivity.
+      Qed.
+
+      Lemma gallina_list_to_idx_to_list_sound : forall attr l rt ,
+          Forall (fun v => type_of_value v (TRecord rt)) l ->
+          In attr (List.map fst rt) ->
+          Permutation (gallina_idx_to_list (gallina_list_to_idx attr l)) l.
+      Proof.
+        intros * H_ty H_in.
+        eapply perm_trans. 2: eapply gallina_list_to_idx_Permutation; eauto.
+        rewrite gallina_idx_to_list__concat_VList_V. 1: apply Permutation_refl.
+        eapply gallina_list_to_idx_shape; eauto.
+      Qed.
+
+      Lemma list_to_idx_to_list_sound :
+        forall attr tbl (Gstore Genv : tenv) (store env : locals) rt,
+          is_NoDup [tup; acc; x; v] ->
+          type_of Gstore Genv tbl (TList (TRecord rt)) ->
+          tenv_wf Gstore -> tenv_wf Genv ->
+          locals_wf Gstore store -> locals_wf Genv env ->
+          In attr (List.map fst rt) ->
+          exists l l',
+            interp_expr store env (idx_to_list (list_to_idx attr tbl)) = VList l /\
+              interp_expr store env tbl = VList l' /\
+              Permutation l l'.
+      Proof.
+        intros * vars_distinct H * H_Gstr H_Genv H_str H_env H_in.
+        eapply type_sound in H as H'; eauto. inversion H'; subst. symmetry in H0.
+        eapply fiat2_gallina_list_to_idx_to_list with (Gstore:=Gstore) (attr:=attr) in H0 as H0'; eauto.
+        repeat eexists; eauto.
+        eapply gallina_list_to_idx_to_list_sound; eauto.
+      Qed.
+
+      Lemma locals_equiv_locals_wf :
+        is_NoDup [tup; acc; x] ->
+        forall x rt attr Gstore' store' store,
+          locals_wf Gstore' store' ->
+          tenv_wf Gstore' ->
+          locals_equiv_idx_list_at x attr store store' ->
+          locals_eq_except x store store' ->
+          map.get Gstore' x = Some (TList (TRecord rt)) ->
+          In attr (List.map fst rt) ->
+          locals_wf (tenv_equiv_at x attr rt Gstore') store.
+      Proof.
+        intro vars_distinct; intros * H_wf H_Gstr' H_equiv H_except H_x H_in. unfold tenv_equiv_at.
+        unfold locals_wf; intros y t. get_put_same_diff x0 y.
+        - intro H_t; injection H_t as H_t; subst.
+          unfold locals_equiv_idx_list_at in H_equiv. repeat destruct_match; intuition.
+          apply H_wf in H_x as H'. rewrite E1 in H'. subst.
+          assert (interp_expr store' map.empty (ELoc y) = VList l0). { simpl; unfold get_local. rewrite E1; auto. }
+          assert (interp_expr store' map.empty (list_to_idx attr (ELoc y)) = VDict (gallina_list_to_idx attr l0)).
+          { eapply fiat2_gallina_list_to_idx with (Genv:=map.empty); eauto.
+            1,3: unfold tenv_wf, locals_wf; intros * contra; rewrite map.get_empty in contra; discriminate.
+            1: constructor; auto. }
+          assert (type_of Gstore' map.empty (ELoc y) (TList (TRecord rt))). { constructor; auto. }
+          eapply list_to_idx_preserve_ty in H1; eauto.
+          1: eapply type_sound with (env:=map.empty) in H1; eauto.
+          2-4: unfold tenv_wf, locals_wf; intros; repeat rewrite map.get_empty in *; discriminate.
+          rewrite H0 in H1. auto.
+        - intro H_y. apply H_wf in H_y. destruct_match; intuition. rewrite H_except; auto. rewrite E0; auto.
+      Qed.
+
+      Hint Resolve locals_equiv_locals_wf : fiat2_hints.
+
+      Definition idx_read_to_list_read (tbl : string) (e : expr) :=
+        match e with
+        | ELoc tbl' => if String.eqb tbl tbl'
+                       then idx_to_list (ELoc tbl)
+                       else e
+        | _ => e
+        end.
+
+      Definition list_write_to_idx_write (tbl attr : string) (c : command) :=
+        match c with
+        | CAssign tbl' e =>
+            if String.eqb tbl tbl'
+            then CAssign tbl (list_to_idx attr e)
+            else c
+        | _ => c
+        end.
+
+      Definition transf_to_idx' (tbl attr : string) (c : command) : command :=
+        fold_command (list_write_to_idx_write tbl attr) (idx_read_to_list_read tbl) c.
+
+      Definition transf_to_idx (tbl attr : string) (c : command) : command :=
+        match c with
+        | CLetMut (EAtom (ANil _)) tbl' c =>
+            CLetMut (EDict nil) tbl (* Rely on can_transf_to_idx to check tbl' = tbl *)
+              (transf_to_idx' tbl attr c)
+        | _ => c
+        end.
+
+      Lemma transf_read_preserve_ty : forall Gstore Genv x attr rt e t,
+          is_NoDup [acc; v] ->
+          tenv_wf Gstore -> tenv_wf Genv ->
+          map.get Gstore x = Some (TList (TRecord rt)) -> type_of Gstore Genv e t ->
+          type_of (tenv_equiv_at x attr rt Gstore) Genv (fold_expr (idx_read_to_list_read x) e) t.
+      Proof.
+        intros * vars_distinct H_Gstr H_Genv H_x H_ty. unfold tenv_equiv_at.
+        generalize dependent Genv. generalize dependent t.
+        induction e using expr_IH; simpl; intros.
+        all: inversion H_ty; subst.
+        all: try now (econstructor; eauto).
+        - get_put_same_diff x0 x1.
+          + rewrite H0 in H_x; injection H_x as H_x; subst.
+            eapply idx_to_list_preserve_ty; eauto with fiat2_hints.
+            constructor. rewrite_map_get_put_goal; f_equal.
+            unfold index_type; eauto.
+          + constructor. rewrite map.get_put_diff; congruence.
+        - econstructor; eauto. apply IHe2; eauto with fiat2_hints.
+        - econstructor; eauto. apply IHe2; auto. eauto with fiat2_hints.
+        - econstructor; eauto. apply IHe3; auto. repeat apply tenv_wf_step; eauto with fiat2_hints.
+        - econstructor; eauto.
+          + rewrite fst_map_fst; auto.
+          + clear H_ty H1 H3 H4 H5. generalize dependent tl. induction l; simpl; intros.
+            1: inversion H2; constructor.
+            destruct tl; simpl in *; inversion H2; subst. constructor; inversion H; subst.
+            1: destruct a; simpl in *; apply H3; auto.
+            apply IHl; auto; injection H1; intros; auto.
+        - econstructor; eauto. clear H_ty. induction H3; intuition. constructor; inversion H; subst.
+          1: destruct x1; simpl in *; split; apply H7; auto.
+          1: apply IHForall; auto.
+        - econstructor; eauto. apply IHe3; eauto with fiat2_hints.
+        - econstructor; eauto. apply IHe3; auto. repeat apply tenv_wf_step; eauto with fiat2_hints.
+        - constructor; auto. apply IHe2; eauto with fiat2_hints.
+        - econstructor; eauto.
+          1: apply IHe3; auto. 2: apply IHe4; eauto with fiat2_hints.
+          all: repeat apply tenv_wf_step; eauto with fiat2_hints.
+        - econstructor; eauto. apply IHe2; eauto with fiat2_hints.
+      Qed.
+
+      Local Ltac apply_transf_read_preserve_ty e attr :=
+        lazymatch goal with
+        | H: type_of _ _ e _ |- _ =>
+            let H_transf_ty := fresh "H_transf_ty" in
+            eapply transf_read_preserve_ty with (attr:=attr) in H as H_transf_ty; eauto with fiat2_hints;
+            apply_type_sound e; try now (simpl in *; intuition);
+            eapply type_sound in H_transf_ty; eauto with fiat2_hints;
+            inversion H_transf_ty; subst
+        end.
+
+      Local Ltac apply_transf_read_write_sound''_IH Gstore' :=
+        lazymatch goal with
+        | H: context[type_of _ _ ?e _ -> _],
+            H_can: can_transf_to_idx'' _ false ?e = true,
+              H_equiv: locals_equiv_idx_list_at _ _ _ _ |- _ =>
+            let IH := fresh "IH" in
+            let IHL := fresh "IHL" in
+            let IH' := fresh "IH'" in
+            eapply H with (Gstore':=Gstore') in H_equiv as IH; eauto; clear H;
+            try (destruct IH as [IHL _]; apply IHL in H_can as IH')
+        | H: context[type_of _ _ ?e _ -> _],
+            H_can: can_transf_to_idx'' _ true ?e = true,
+              H_equiv: locals_equiv_idx_list_at _ _ _ _ |- _ =>
+            let IH := fresh "IH" in
+            let IHR := fresh "IHR" in
+            let IH' := fresh "IH'" in
+            eapply H with (Gstore':=Gstore') in H_equiv as IH; eauto; clear H;
+            try (destruct IH as [_ IHR]; apply IHR in H_can as IH')
+        end.
+
+      Lemma transf_read_write_sound'' : forall tbl attr rt e Gstore' Genv t store store' env,
+          is_NoDup [tup; acc; x; v] ->
+          type_of Gstore' Genv e t ->
+          tenv_wf Gstore' -> tenv_wf Genv ->
+          map.get Gstore' tbl = Some (TList (TRecord rt)) -> In attr (List.map fst rt) ->
+          locals_wf Gstore' store' -> locals_wf Genv env ->
+          locals_eq_except tbl store store' ->
+          locals_equiv_idx_list_at tbl attr store store' ->
+          (can_transf_to_idx'' tbl false e -> interp_expr store env (fold_expr (idx_read_to_list_read tbl) e) = interp_expr store' env e) /\
+            (can_transf_to_idx'' tbl true e ->
+             match t with
+             | TList t =>
+                 match interp_expr store env (fold_expr (idx_read_to_list_read tbl) e) with
+                 | VList l => match interp_expr store' env e with
+                              | VList l' => Permutation l l'
+                              | _ => False
+                              end
+                 | _ => False
+                 end
+             | _ => interp_expr store env (fold_expr (idx_read_to_list_read tbl) e) = interp_expr store' env e
+             end).
+      Proof.
+        induction e using expr_IH; cbn; intros * vars_distinct H_ty H_Gstr' H_Genv H_tbl_ty H_in H_str' H_env H_except H_equiv; auto.
+        - (* EVar *)
+          split; intros; auto. apply_type_sound (EVar x0).
+        - (* ELoc *)
+          split; intros.
+          all: unfold is_true in *; rewrite Bool.orb_true_iff in H.
+          + destruct (String.eqb x0 tbl) eqn:E; intuition; try discriminate.
+            rewrite eqb_sym; rewrite E; try discriminate. apply eqb_neq in E. simpl.
+            unfold get_local. rewrite H_except; auto.
+          +  clear H; destruct (String.eqb x0 tbl) eqn:E; rewrite eqb_sym; rewrite E.
+             * (* x0 = tbl *) rewrite eqb_eq in E; subst.
+               inversion H_ty; subst. rewrite H0 in H_tbl_ty. injection H_tbl_ty; intros; subst.
+               apply_type_sound (ELoc tbl).
+               erewrite fiat2_gallina_idx_to_list with (Gstore:=tenv_equiv_at tbl attr rt Gstore'); simpl; eauto with fiat2_hints.
+               1: eapply gallina_list_to_idx_to_list_sound; eauto.
+               1: intuition.
+               1:{ constructor. unfold tenv_equiv_at. rewrite map.get_put_same. eauto. }
+               1:{ unfold get_local. eapply locals_equiv_locals_wf; eauto. simpl in *; intuition. }
+               1:{ unfold locals_equiv_idx_list_at in H_equiv; repeat destruct_match; intuition.
+                   subst. unfold get_local in *. rewrite E1 in H. rewrite E. injection H; congruence. }
+             * (* x <> tbl *) rewrite eqb_neq in E. destruct t; simpl.
+               all: unfold get_local; rewrite H_except; auto.
+               apply_type_sound (ELoc x0). unfold get_local in *.
+               rewrite_expr_value. intuition.
+        - (* EAtom *)
+          split; intro H_can; destruct t; auto. inversion H_ty; subst. invert_unop_binop_atom_ty.
+          all: simpl; intuition.
+        - (* EUnop *)
+          inversion H_ty; subst. split; intro H_can; destruct o; simpl in *.
+          all: invert_unop_binop_atom_ty; unfold is_true in H_can.
+          all: apply_transf_read_write_sound''_IH Gstore'; try rewrite IH'; auto.
+          (* OLength *)
+          all: apply_transf_read_preserve_ty e attr.
+          all: [> iter_hyps rewrite_hyp_l ..].
+          all: destruct_match; intuition; erewrite Permutation_length; eauto.
+        - (* EBinop *)
+          inversion H_ty; subst. split; intro H_can; destruct o; simpl in *.
+          all: invert_unop_binop_atom_ty; unfold is_true in H_can; repeat rewrite Bool.andb_true_iff in H_can.
+          all: try (intuition; repeat apply_transf_read_write_sound''_IH Gstore'; try congruence; intuition;
+                    repeat rewrite_interp_fold_expr; try congruence; intuition).
+          1,2,4,5: (* OConcat, ORepeat, ORange, OWRange *)
+            apply_type_sound e1; apply_type_sound e2; auto.
+          (* OCons *)
+          eapply locals_equiv_locals_wf in H_equiv as H_wf; eauto. 2: simpl; intuition.
+          apply_transf_read_preserve_ty e2 attr. destruct_match; intuition.
+          apply perm_skip. repeat rewrite_expr_value; auto.
+        - (* EIf *)
+          inversion H_ty; subst. split; intro H_can.
+          all: unfold is_true in H_can; repeat rewrite Bool.andb_true_iff in H_can; intuition.
+          all: repeat apply_transf_read_write_sound''_IH Gstore'; simpl; intuition;
+            repeat rewrite_interp_fold_expr; auto.
+          apply_type_sound e1. destruct b; auto.
+        - (* ELet *)
+          inversion H_ty; subst. split; intro H_can.
+          all: unfold is_true in H_can; repeat rewrite Bool.andb_true_iff in H_can; intuition.
+          all: repeat apply_transf_read_write_sound''_IH Gstore'; simpl; intuition;
+            repeat rewrite_interp_fold_expr; eauto with fiat2_hints.
+        - (* EFlatmap *)
+          inversion H_ty; subst. split; intro H_can.
+          all: unfold is_true in H_can; repeat rewrite Bool.andb_true_iff in H_can; intuition.
+          all: revert IHe2; apply_transf_read_write_sound''_IH Gstore'; simpl; intuition; intros.
+          + rewrite_interp_fold_expr; auto. apply_type_sound e1. f_equal.
+            apply In_flat_map_ext. intros a H_a_in. apply_transf_read_write_sound''_IH Gstore'; try rewrite_interp_fold_expr; eauto with fiat2_hints.
+            1: intuition.
+            apply locals_wf_step; auto; apply_Forall_In.
+          + eapply locals_equiv_locals_wf in H_equiv as H_wf; eauto.
+            2: simpl; intuition.
+            apply_transf_read_preserve_ty e1 attr; repeat rewrite_expr_value.
+            destruct_match; auto. apply Permutation_flat_map; auto.
+            intros v0 H_v_in. eapply Permutation_in in H_v_in; eauto. apply_Forall_In.
+            apply_transf_read_write_sound''_IH Gstore'; eauto with fiat2_hints; intuition.
+            apply_transf_read_preserve_ty e2 attr; eauto with fiat2_hints.
+            iter_hyps rewrite_hyp_l; auto. destruct_match; intuition.
+        - (* EFold *)
+          inversion H_ty; subst.
+          apply imp_pre_true.
+          1: intro H_can.
+          2: intros HA H_can; specialize (HA H_can).
+          all: unfold is_true in H_can; repeat rewrite Bool.andb_true_iff in H_can; intuition.
+          all: revert IHe3; repeat apply_transf_read_write_sound''_IH Gstore'; intros; simpl; intuition.
+          + repeat rewrite_interp_fold_expr. apply_type_sound e1.
+            eapply type_sound in H6 as H2'; eauto.
+            eapply In_fold_right_ext with (P:=fun a => type_of_value a t); auto.
+            intros * P H_b_in. intuition.
+            1:{ apply_transf_read_write_sound''_IH Gstore'; eauto; simpl; intuition.
+                1: repeat apply tenv_wf_step; eauto with fiat2_hints.
+                1: repeat apply locals_wf_step; eauto with fiat2_hints; apply_Forall_In. }
+            1:{ apply_transf_read_write_sound''_IH Gstore'; auto; simpl; intuition.
+                1: rewrite_interp_fold_expr; eapply type_sound; eauto.
+                1,3: repeat apply tenv_wf_step; eauto with fiat2_hints.
+                1,2: repeat apply locals_wf_step; eauto with fiat2_hints; apply_Forall_In. }
+          + rewrite HA. destruct t; auto.
+            apply_type_sound (EFold e1 e2 x0 y e3).
+        - (* ERecord *)
+          inversion H_ty; subst. split; intro H_can.
+          all: unfold is_true in H_can; repeat rewrite Bool.andb_true_iff in H_can; intuition.
+          all: do 2 f_equal; rewrite map_map.
+          all: apply In_map_ext; intros x0 H_x_in; apply_Forall_In;
+            rewrite forallb_forall in H_can; apply H_can in H_x_in as H_x.
+          all: apply in_map with (f:=snd) in H_x_in; pose proof (Forall2_In_Permuted _ _ _ _ _ _ H2 H_x_in).
+          all: do 3 lazymatch goal with H: exists _, _ |- _ => destruct H end; intuition.
+          all: eapply H with (Gstore':=Gstore') in H_equiv as IH; eauto; simpl; intuition.
+          all: destruct x0; simpl in *; congruence.
+        - (* EAccess *)
+          inversion H_ty; subst. split; intro H_can.
+          all: unfold is_true in H_can; repeat rewrite Bool.andb_true_iff in H_can; intuition.
+          all: apply_transf_read_write_sound''_IH Gstore'; simpl; intuition; rewrite_interp_fold_expr; auto.
+          destruct t; auto. apply_type_sound (EAccess e s).
+        - (* EDict *)
+          inversion H_ty; subst. split; intro H_can.
+          all: unfold is_true in H_can.
+          all: do 3 f_equal; rewrite map_map; apply In_map_ext.
+          all: intros x0 H_x_in; destruct x0; simpl in *.
+          all: repeat apply_Forall_In; rewrite forallb_forall in H_can; apply H_can in H_x_in as H_x.
+          all: repeat rewrite Bool.andb_true_iff in *; intuition; simpl in *.
+          all: repeat apply_transf_read_write_sound''_IH Gstore'; simpl; intuition.
+          all: rewrite IH', IH'0; auto.
+        - (* EInsert *)
+          inversion H_ty; subst. split; intro H_can.
+          all: unfold is_true in H_can; repeat rewrite Bool.andb_true_iff in H_can; intuition.
+          all: repeat apply_transf_read_write_sound''_IH Gstore'; repeat rewrite_interp_fold_expr; auto.
+          all: simpl; intuition.
+        - (* EDelete *)
+          inversion H_ty; subst. split; intro H_can.
+          all: unfold is_true in H_can; repeat rewrite Bool.andb_true_iff in H_can; intuition.
+          all: repeat apply_transf_read_write_sound''_IH Gstore'; repeat rewrite_interp_fold_expr; auto.
+          all: simpl; intuition.
+        - (* ELookup *)
+          inversion H_ty; subst. split; intro H_can.
+          all: unfold is_true in H_can; repeat rewrite Bool.andb_true_iff in H_can; intuition.
+          all: repeat apply_transf_read_write_sound''_IH Gstore'; repeat rewrite_interp_fold_expr; auto.
+          all: simpl; intuition.
+        - (* EOptMatch *)
+          inversion H_ty; subst. split; intro H_can.
+          all: unfold is_true in H_can; repeat rewrite Bool.andb_true_iff in H_can; intuition.
+          all: revert IHe2 IHe3; apply_transf_read_write_sound''_IH Gstore'; simpl; intuition; intros.
+          all: rewrite_interp_fold_expr; apply_type_sound e1.
+          all: try now (revert IHe3; apply_transf_read_write_sound''_IH Gstore'; eauto; intuition).
+          all: revert IHe2; apply_transf_read_write_sound''_IH Gstore'; eauto with fiat2_hints; intuition.
+        - (* EDictFold *)
+          inversion H_ty; subst. apply imp_pre_true.
+          1: intro H_can.
+          2: intros HA H_can; specialize (HA H_can).
+          all: unfold is_true in H_can; repeat rewrite Bool.andb_true_iff in H_can; intuition.
+          all: revert IHe3; repeat apply_transf_read_write_sound''_IH Gstore'; simpl; intuition; intros.
+          + repeat rewrite_interp_fold_expr; apply_type_sound e1.
+            apply In_fold_right_ext with (P := fun a => type_of_value a t).
+            2:{ intros. apply_transf_read_write_sound''_IH Gstore'; intuition.
+                1: rewrite_interp_fold_expr; auto.
+                2: repeat apply tenv_wf_step; eauto with fiat2_hints.
+                2: repeat apply locals_wf_step; auto; apply_Forall_In; intuition.
+                eapply type_sound with (Gstore:=tenv_equiv_at tbl attr rt Gstore').
+                1: apply transf_read_preserve_ty; simpl; intuition. 2: eauto.
+                2: apply tenv_equiv_at_wf; auto. 3: eapply locals_equiv_locals_wf; eauto; simpl; intuition.
+                1-2: repeat apply tenv_wf_step; eauto with fiat2_hints.
+                1: repeat apply locals_wf_step; apply_Forall_In; intuition. }
+            apply_type_sound e2; eauto.
+          + rewrite HA. destruct t; auto.
+            apply_type_sound (EDictFold e1 e2 k0 v0 acc0 e3).
+        - (* ESort *)
+          inversion H_ty; subst. split; intro H_can.
+          all: unfold is_true in H_can; repeat rewrite Bool.andb_true_iff in H_can; intuition.
+          all: apply_transf_read_write_sound''_IH Gstore'; simpl; intuition.
+          1:{ repeat destruct_match; intuition. f_equal. apply Permutation_SSorted_eq; auto using StronglySorted_value_sort.
+              pose proof Permuted_value_sort l. pose proof Permuted_value_sort l0.
+              eapply perm_trans. 2: eauto. apply Permutation_sym. eapply perm_trans. 2: eauto. apply Permutation_sym; auto. }
+          1:{ eapply locals_equiv_locals_wf in H_equiv as H_wf; eauto; simpl; intuition.
+              apply_transf_read_preserve_ty e attr. repeat rewrite_expr_value.
+              pose proof Permuted_value_sort l. destruct_match; intuition. pose proof Permuted_value_sort l0.
+              eapply perm_trans. 2: eauto. apply Permutation_sym. eapply perm_trans. 2: eauto. apply Permutation_sym; auto. }
+        - (* EFilter *)
+          inversion H_ty; subst. split; intro H_can.
+          all: unfold is_true in H_can; repeat rewrite Bool.andb_true_iff in H_can; intuition.
+          all: revert IHe2; apply_transf_read_write_sound''_IH Gstore'; simpl; intuition; intros.
+          + rewrite_interp_fold_expr. apply_type_sound e1. f_equal.
+            apply filter_ext_in; intros a H_a_in. apply_transf_read_write_sound''_IH Gstore'; eauto with fiat2_hints; intuition.
+            1: rewrite_interp_fold_expr; auto.
+            1: apply locals_wf_step; auto; apply_Forall_In.
+          + eapply locals_equiv_locals_wf in H_equiv as H_wf; eauto; simpl; intuition.
+            apply_transf_read_preserve_ty e1 attr. repeat destruct_match; intuition. repeat rewrite_expr_value.
+            rewrite In_filter_ext with
+              (g:=fun v : value => match interp_expr store' (map.put env x0 v) e2 with
+                                   | VBool b => b
+                                   | _ => false
+                                   end).
+            2:{ intros a H_a_in. apply_transf_read_write_sound''_IH Gstore'; eauto with fiat2_hints; intuition.
+                1: rewrite_interp_fold_expr; auto.
+                1:{ apply locals_wf_step; auto. do_injection. eapply Permutation_in in H_a_in; eauto. apply_Forall_In. }}
+            apply Permutation_filter; congruence.
+        - (* EJoin *)
+          inversion H_ty; subst. split; intro H_can.
+          all: unfold is_true in H_can; repeat rewrite Bool.andb_true_iff in H_can; intuition.
+          all: revert IHe3 IHe4; repeat apply_transf_read_write_sound''_IH Gstore'; simpl; intuition; intros.
+          + repeat rewrite_interp_fold_expr.
+            apply_type_sound e1. apply_type_sound e2. f_equal.
+            apply In_flat_map_ext; intros a H_a_in.
+            rewrite In_filter_ext with
+              (g:=fun v2 : value => match interp_expr store' (map.put (map.put env x0 a) y v2) e3 with
+                                    | VBool b => b
+                                    | _ => false
+                                    end).
+            1: apply In_map_ext; intros b H_b_in; revert IHe3; repeat apply_transf_read_write_sound''_IH Gstore'; auto; intuition.
+            1: repeat apply tenv_wf_step; eauto with fiat2_hints.
+            1: repeat apply locals_wf_step; eauto with fiat2_hints.
+            1,2: rewrite filter_In in H_b_in; intuition; repeat apply_Forall_In.
+            intros c H_c_in. revert IHe4; apply_transf_read_write_sound''_IH Gstore'; simpl; intuition; intros.
+            1: rewrite_interp_fold_expr; auto.
+            1: repeat apply tenv_wf_step; eauto with fiat2_hints.
+            1: repeat apply locals_wf_step; repeat apply_Forall_In.
+          + eapply locals_equiv_locals_wf in H_equiv as H_wf; eauto; simpl; intuition.
+            apply_transf_read_preserve_ty e1 attr.
+            apply_transf_read_preserve_ty e2 attr. repeat destruct_match; intuition. repeat rewrite_expr_value.
+            repeat (try clear_refl; repeat do_injection). auto. apply Permutation_flat_map; auto.
+            intros a H_a_in.
+            rewrite In_map_ext with (g:=fun v2 : value => interp_expr store' (map.put (map.put env x0 a) y v2) e4).
+            1: apply Permutation_map.
+            1: rewrite In_filter_ext with
+              (g:=fun v2 : value => match interp_expr store' (map.put (map.put env x0 a) y v2) e3 with
+                                    | VBool b => b
+                                    | _ => false
+                                    end).
+            1:{ apply Permutation_filter; auto. }
+            1:{ intros b H_b_in. revert IHe4; apply_transf_read_write_sound''_IH Gstore'; simpl; intuition; intros.
+                1: rewrite_interp_fold_expr; auto.
+                1: repeat apply tenv_wf_step; eauto with fiat2_hints.
+                1: repeat apply locals_wf_step; auto;
+                eapply Permutation_in in H_a_in, H_b_in; eauto; repeat apply_Forall_In. }
+            1:{ intros b H_b_in. revert IHe3; apply_transf_read_write_sound''_IH Gstore'; simpl; intuition; intros.
+                1: rewrite_interp_fold_expr; auto.
+                1: repeat apply tenv_wf_step; eauto with fiat2_hints.
+                1: repeat apply locals_wf_step; auto.
+                1,2: apply filter_In in H_b_in; intuition.
+                1: eapply Permutation_in in H_a_in; eauto; apply_Forall_In.
+                1: eapply Permutation_in in H20; eauto; apply_Forall_In. }
+        - (* EProj *)
+          inversion H_ty; subst. split; intro H_can.
+          all: unfold is_true in H_can; repeat rewrite Bool.andb_true_iff in H_can; intuition.
+          all: revert IHe2; apply_transf_read_write_sound''_IH Gstore'; simpl; intuition; intros.
+          + rewrite_interp_fold_expr. apply_type_sound e1. f_equal. apply In_map_ext.
+            intros a H_a_in. apply_transf_read_write_sound''_IH Gstore'; eauto with fiat2_hints; simpl; intuition.
+            repeat apply locals_wf_step; apply_Forall_In.
+          + eapply locals_equiv_locals_wf in H_equiv as H_wf; eauto; simpl; intuition.
+            apply_transf_read_preserve_ty e1 attr. repeat destruct_match; intuition. do_injection.
+            rewrite In_map_ext with (g:=(fun v : value => interp_expr store' (map.put env x0 v) e2)).
+            2:{ intros a H_a_in. apply_transf_read_write_sound''_IH Gstore'; eauto with fiat2_hints; simpl; intuition.
+                repeat apply locals_wf_step; auto. eapply Permutation_in in H_a_in; eauto. apply_Forall_In. }
+            repeat rewrite_expr_value. apply Permutation_map; auto.
+      Qed.
+
+      Lemma transf_read_write_sound' : forall c Gstore' Genv rt store store' env tbl attr,
+          is_NoDup [tup; acc; x; v] ->
+          well_typed Gstore' Genv c ->
+          map.get Gstore' tbl = Some (TList (TRecord rt)) ->
+          In attr (List.map fst rt) ->
+          tenv_wf Gstore' -> tenv_wf Genv -> locals_wf Gstore' store' -> locals_wf Genv env ->
+          locals_eq_except tbl store store' ->
+          locals_equiv_idx_list_at tbl attr store store' ->
+          can_transf_to_idx' tbl c = true ->
+          (locals_eq_except tbl
              (interp_command store env (transf_to_idx' tbl attr c))
-             (interp_command store' env c)).
-    Proof.
-      induction c; simpl; auto; intros * H_ty H_tbl_ty H_in H_Gstr' H_Genv H_str' H_env H_except H_equiv H_can.
-      all: repeat rewrite Bool.andb_true_iff in H_can; inversion H_ty; subst.
-      - eapply IHc2; try eapply IHc1; eauto; intuition.
-        eapply command_type_sound; eauto.
-      - destruct H_can.
-        eapply transf_read_write_sound'' with (Gstore':=Gstore') in H as H'; eauto. rewrite H'.
-        eapply IHc; eauto; [ apply tenv_wf_step | apply locals_wf_step ]; eauto with fiat2_hints.
-      - rewrite Bool.negb_true_iff, eqb_neq in *.
-        assert (E: map.get store x = map.get store' x). { apply H_except; intuition. } rewrite E.
-        repeat lazymatch goal with H: _ /\ _ |- _ => destruct H end.
-        eapply transf_read_write_sound'' with (Gstore':=Gstore') in H2 as H'; eauto. rewrite H'.
-        split. 1: apply locals_eq_except_update. 2: apply locals_equiv_idx_list_at_update. 3: congruence.
-        1,2: eapply IHc; eauto with fiat2_hints. all: rewrite map.get_put_diff; auto.
-      - cbn. eapply transf_read_write_sound'' with (Gstore':=Gstore') in H_can; eauto.
-        destruct (String.eqb tbl x) eqn:E.
-        + unfold fold_command. unfold interp_command.
-          rewrite eqb_eq in *; subst. rewrite H_tbl_ty in H1. injection H1; intros; subst.
+             (interp_command store' env c)) /\
+            (locals_equiv_idx_list_at tbl attr
+               (interp_command store env (transf_to_idx' tbl attr c))
+               (interp_command store' env c)).
+      Proof.
+        induction c; simpl; auto; intros * vars_distinct H_ty H_tbl_ty H_in H_Gstr' H_Genv H_str' H_env H_except H_equiv H_can.
+        all: repeat rewrite Bool.andb_true_iff in H_can; inversion H_ty; subst.
+        - eapply IHc2; try eapply IHc1; eauto; intuition.
+          eapply command_type_sound; eauto.
+        - destruct H_can.
+          eapply transf_read_write_sound'' with (Gstore':=Gstore') in H as H'; eauto. rewrite H'.
+          eapply IHc; eauto; [ apply tenv_wf_step | apply locals_wf_step ]; eauto with fiat2_hints.
+        - rewrite Bool.negb_true_iff, eqb_neq in *.
+          assert (E: map.get store x0 = map.get store' x0). { apply H_except; intuition. } rewrite E.
+          repeat lazymatch goal with H: _ /\ _ |- _ => destruct H end.
+          eapply transf_read_write_sound'' with (Gstore':=Gstore') in H2 as H'; eauto.
+          2: simpl; intuition.
+          rewrite H'. split.
+          1: apply locals_eq_except_update. 2: apply locals_equiv_idx_list_at_update. 3: congruence.
+          1,2: eapply IHc; eauto with fiat2_hints. all: simpl; intuition; rewrite map.get_put_diff; auto.
+        - cbn. eapply transf_read_write_sound'' with (Gstore':=Gstore') in H_can; eauto.
+          destruct (String.eqb tbl x0) eqn:E.
+          + unfold fold_command. unfold interp_command.
+            rewrite eqb_eq in *; subst. rewrite H_tbl_ty in H1. injection H1; intros; subst.
+            apply_type_sound e.
+            split; eauto with fiat2_hints. eapply locals_equiv_idx_list_at_put0; eauto.
+            remember (map.put Gstore' x0 (index_type (get_attr_type rt attr) rt)) as Gstore.
+            eapply fiat2_gallina_list_to_idx with (Gstore:=Gstore); eauto; simpl; intuition.
+            1:{ subst. apply tenv_wf_step; auto. apply type_of__type_wf in H2; auto. inversion H2; subst. inversion H15; subst. repeat constructor; simpl; eauto with fiat2_hints. intuition; congruence. }
+            1: subst; apply transf_read_preserve_ty; auto; simpl; intuition.
+            1: subst; eapply locals_equiv_locals_wf; eauto; simpl; intuition.
+            1: rewrite H_can; auto.
+          + simpl. rewrite H_can.
+            rewrite eqb_neq in *. split; auto with fiat2_hints.
+        - repeat lazymatch goal with H: _ /\ _ |- _ => destruct H end.
+          eapply transf_read_write_sound'' with (Gstore':=Gstore') in H; eauto.
+          2: simpl; intuition. rewrite H.
+          apply_type_sound e. destruct b; [ eapply IHc1 | eapply IHc2 ]; eauto; simpl; intuition.
+        - repeat lazymatch goal with H: _ /\ _ |- _ => destruct H end.
+          eapply transf_read_write_sound'' with (Gstore':=Gstore') in H; eauto.
+          2: simpl; intuition. rewrite H.
           apply_type_sound e.
-          split; eauto with fiat2_hints. eapply locals_equiv_idx_list_at_put0; eauto.
-          remember (map.put Gstore' x (TDict (get_attr_type rt attr) (TList (TRecord rt)))) as Gstore.
-          eapply fiat2_gallina_list_to_idx with (Gstore:=Gstore); eauto.
-          1: subst; apply transf_read_preserve_ty; auto.
-          1:{ subst. apply tenv_wf_step; auto. apply type_of__type_wf in H2; auto. constructor; eauto with fiat2_hints. }
-          1: subst; eapply locals_equiv_locals_wf; eauto.
-          1: rewrite H_can; auto.
-        + simpl. rewrite H_can.
-          rewrite eqb_neq in *. split; auto with fiat2_hints.
-      - repeat lazymatch goal with H: _ /\ _ |- _ => destruct H end.
-        eapply transf_read_write_sound'' with (Gstore':=Gstore') in H; eauto. rewrite H.
-        apply_type_sound e. destruct b; eauto.
-      - repeat lazymatch goal with H: _ /\ _ |- _ => destruct H end.
-        eapply transf_read_write_sound'' with (Gstore':=Gstore') in H; eauto. rewrite H.
-        apply_type_sound e.
-        destruct (interp_expr store' env e) eqn:E; try now (exfalso; auto).
-        clear E H H2. generalize dependent store; generalize dependent store'. induction l; simpl; auto. intros.
-        lazymatch goal with H: Forall _ (_ :: _) |- _ => inversion H; subst end. apply IHl; auto.
-        1: eapply command_type_sound; eauto.
-        3,4: eapply IHc.
-        all: eauto with fiat2_hints.
-    Qed.
+          destruct (interp_expr store' env e) eqn:E; try now (exfalso; auto).
+          clear E H H8. generalize dependent store; generalize dependent store'. induction l; simpl; auto. intros.
+          lazymatch goal with H: Forall _ (_ :: _) |- _ => inversion H; subst end. apply IHl; auto.
+          1: eapply command_type_sound; eauto.
+          3,4: eapply IHc.
+          all: eauto with fiat2_hints; simpl; intuition.
+      Qed.
 
-    Lemma transf_read_write_sound : forall (Gstore Genv : tenv) (store env : locals) tbl attr c,
-        tenv_wf Gstore -> tenv_wf Genv ->
-        well_typed Gstore Genv c ->
-        locals_wf Gstore store -> locals_wf Genv env ->
-        can_transf_to_idx tbl attr c = true ->
-        interp_command store env (transf_to_idx tbl attr c) = interp_command store env c.
-    Proof.
-      intros * H_Gstr H_Genv H_ty H_str H_env H.
-      destruct c; simpl in *; try discriminate.
+      Lemma transf_read_write_sound : forall (Gstore Genv : tenv) (store env : locals) tbl attr c,
+          is_NoDup [tup; acc; x; v] ->
+          tenv_wf Gstore -> tenv_wf Genv ->
+          well_typed Gstore Genv c ->
+          locals_wf Gstore store -> locals_wf Genv env ->
+          can_transf_to_idx tbl attr c = true ->
+          interp_command store env (transf_to_idx tbl attr c) = interp_command store env c.
+      Proof.
+        intros * vars_distinct H_Gstr H_Genv H_ty H_str H_env H.
+        destruct c; simpl in *; try discriminate.
       repeat (destruct_match; try discriminate).
-      repeat rewrite Bool.andb_true_iff in H; intuition.
-      apply eqb_eq in H; subst; simpl. apply locals_eq_update. intros.
+      repeat rewrite Bool.andb_true_iff in H.
+      do 2 destruct H. apply eqb_eq in H; subst; simpl. apply locals_eq_update. intros.
       inversion H_ty; subst. inversion H4; subst. inversion H3; subst.
-      eapply transf_read_write_sound'; cbn; eauto with fiat2_hints.
+      eapply transf_read_write_sound'; cbn; eauto with fiat2_hints; intuition.
       - rewrite map.get_put_same; eauto.
       - rewrite inb_true_iff in *; auto.
       - apply locals_wf_step; auto. repeat constructor.
@@ -1224,78 +1336,25 @@ Section WithWord.
       - unfold locals_equiv_idx_list_at. repeat rewrite map.get_put_same; trivial.
     Qed.
 
-    Definition eq_filter_to_lookup_head (tbl attr : string) (e : expr) :=
-      match e with
-      | EFilter
-          (EDictFold (ELoc tbl') (EAtom (ANil None)) k v acc (EBinop OConcat (EVar v') (EVar acc')))
-          x
-          (EBinop OEq (EAccess (EVar y) attr') e') =>
-          if (String.eqb k "k" && String.eqb v "v" && String.eqb v v' && String.eqb acc "acc" && String.eqb acc acc' && String.eqb tbl' tbl && String.eqb attr' attr && String.eqb x y &&
-                negb (String.eqb v' acc') && negb (free_immut_in x e'))%bool
-          then EOptMatch (ELookup (ELoc tbl) e')
-                 (EAtom (ANil None))
-                 "x" (EVar "x")
-          else e
-      | _ => e
+    Lemma fold_idx_to_list : forall idx,
+        EDictFold idx enil k v acc
+          (EBinop OConcat (ofst (EVar v))
+             (econs (osnd (EVar v)) (EVar acc))) = idx_to_list idx.
+    Proof. reflexivity. Qed.
+    End list_idx.
+
+    (* Every string in l equals s *)
+    Fixpoint all_eqb' (s : string) (l : list string) : bool :=
+      match l with
+      | nil => true
+      | x :: l => String.eqb x s && all_eqb' s l
       end.
 
-    Local Ltac invert_type_of :=
-      lazymatch goal with
-      | H: type_of _ _ (_ _) _ |- _ => inversion H; subst; clear H
-      | H: type_of_binop _ _ _ _ |- _ => inversion H; subst; clear H
+    Fixpoint all_eqb (l : list (string * list string)) : bool :=
+      match l with
+      | nil => true
+      | (s, sl) :: l => all_eqb' s sl && all_eqb l
       end.
-
-    Local Ltac rewrite_map_get_put :=
-      lazymatch goal with
-      | H: context[map.get (map.put _ ?x _) ?x] |- _ =>
-          rewrite map.get_put_same in H
-      | H: context[map.get (map.put _ _ _) _] |- _ =>
-          rewrite map.get_put_diff in H; try congruence
-      | |- context[map.get (map.put _ ?x _) ?x] =>
-          rewrite map.get_put_same
-      | |- context[map.get (map.put _ _ _) _] =>
-          rewrite map.get_put_diff; try congruence
-      end.
-
-    Local Ltac clear_refl := lazymatch goal with H: ?x = ?x |- _ => clear H end.
-
-    Local Ltac do_injection :=
-      lazymatch goal with
-      | H: ?c _ = ?c _ |- _ => injection H; intros; subst
-      end.
-
-    Lemma eq_filter_to_lookup_head_preserve_ty : forall tbl attr e rt t (Gstore Genv : tenv),
-        tenv_wf Gstore -> tenv_wf Genv ->
-        map.get Gstore tbl = Some (TDict (get_attr_type rt attr) (TList (TRecord rt))) ->
-        type_of Gstore Genv e t ->
-        type_of Gstore Genv (eq_filter_to_lookup_head tbl attr e) t.
-    Proof.
-      intros * H_Gstr H_Genv H_tbl_ty H.
-      destruct e; auto. destruct e1; auto. destruct e1_1; auto. destruct e1_2; auto.
-      destruct a; auto. destruct t0; auto. destruct e1_3; auto. destruct o; auto.
-      destruct e1_3_1; auto. destruct e1_3_2; auto. destruct e2; auto. destruct o; auto.
-      destruct e2_1; auto. destruct e2_1; auto. simpl.
-      lazymatch goal with |- context[if ?x then _ else _] => destruct x eqn:E end; auto.
-      repeat rewrite Bool.andb_true_iff in E; intuition. rewrite Bool.negb_true_iff, eqb_eq, eqb_neq in *; subst.
-      repeat invert_type_of. repeat rewrite_map_get_put.
-      injection H5; intro; subst.
-      repeat econstructor; eauto.
-      1:{ rewrite H10 in H_tbl_ty. repeat (clear_refl; repeat do_injection).
-          unfold get_attr_type. repeat (clear_refl; repeat do_injection). rewrite H7.
-          eapply not_free_immut_put_ty; eauto. }
-      1:{ rewrite map.get_put_same; trivial. }
-    Qed.
-
-    Definition index_wf (attr : string) (l : list (value * value)) :=
-      NoDup (List.map fst l) /\
-        Forall (fun p => match snd p with
-                         | VList l =>
-                             Forall (fun r => match r with
-                                              | VRecord r => access_record r attr = Success (fst p)
-                                              | _ => False
-                                              end) l
-                         | _ => False
-                         end) l.
 
     Definition gallina_filter_access_eq (s : string) (v0 : value) (l : list value) :=
       filter (fun v => value_eqb match v with
@@ -1309,9 +1368,86 @@ Section WithWord.
         free_immut_in x e2 = false ->
         interp_expr store env (EFilter e1 x (EBinop OEq (EAccess (EVar x) s) e2)) =
           VList (gallina_filter_access_eq s (interp_expr store env e2) l).
+    Proof.
+      intros * H1 H_free; simpl. rewrite H1. f_equal. apply filter_ext. intro a.
+      unfold get_local. rewrite map.get_put_same. rewrite <- not_free_immut_put_sem; auto.
+    Qed.
+
+    Lemma Forall_false__filter : forall A f (l : list A), Forall (fun x => f x = false) l -> filter f l = nil.
+    Proof.
+      intros * H; induction l; simpl; auto. simpl in H.
+      inversion H; subst. rewrite H2. auto.
+    Qed.
+
+    Section eq_filter_to_lookup.
+      Context (k v acc p : string).
+
+      Definition nodup_vars := is_NoDup [k; v; acc; p].
+
+      Definition eq_filter_to_lookup_head (tbl attr : string) (e : expr) :=
+        (* filter (idx_to_list idx) (fun row => row.attr == e') -->
+           match (lookup idx e') with none => nil | some p => fst p ++ [snd p] *)
+        match e with
+        | EFilter
+            (EDictFold (ELoc tbl0) (EAtom (ANil None)) k0 v0 acc0
+               (EBinop OConcat
+                  (EAccess (EVar v1) "0")
+                  (EBinop OCons (EAccess (EVar v2) "1") (EVar acc1))))
+            x
+            (EBinop OEq (EAccess (EVar x0) attr0) e') =>
+            if (all_eqb [(k, [k0]); (v, [v0; v1; v2]); (acc, [acc0; acc1]); (tbl, [tbl0]); (attr, [attr0]); (x, [x0])] &&
+                  negb (String.eqb v acc) && negb (free_immut_in x e'))%bool
+            then EOptMatch (ELookup (ELoc tbl) e')
+                   enil
+                   p (EBinop OConcat (ofst (EVar p)) (econs (osnd (EVar p)) enil))
+            else e
+        | _ => e
+        end.
+
+      Lemma eq_filter_to_lookup_head_preserve_ty : forall tbl attr e rt t (Gstore Genv : tenv),
+          nodup_vars ->
+          tenv_wf Gstore -> tenv_wf Genv ->
+          map.get Gstore tbl = Some (index_type (get_attr_type rt attr) rt) ->
+          type_of Gstore Genv e t ->
+          type_of Gstore Genv (eq_filter_to_lookup_head tbl attr e) t.
       Proof.
-        intros * H1 H_free; simpl. rewrite H1. f_equal. apply filter_ext. intro a.
-        unfold get_local. rewrite map.get_put_same. rewrite <- not_free_immut_put_sem; auto.
+        intros * vars_distinct H_Gstr H_Genv H_tbl_ty H_ty.
+        repeat destruct_subexpr. simpl.
+        lazymatch goal with |- context[if ?x then _ else _] => destruct x eqn:E end; auto. repeat rewrite Bool.andb_true_r in E.
+      repeat rewrite Bool.andb_true_iff in E; intuition. rewrite Bool.negb_true_iff, eqb_eq, eqb_neq in *; subst.
+      repeat invert_type_of. repeat rewrite_map_get_put_hyp.
+      repeat (clear_refl; repeat do_injection).
+      repeat (econstructor; eauto).
+      1:{ rewrite H12 in H_tbl_ty. do_injection. simpl in *; do_injection.
+          unfold get_attr_type. rewrite H7.
+          eapply not_free_immut_put_ty; eauto. }
+      all: rewrite map.get_put_same; trivial.
+    Qed.
+
+    Definition index_wf (attr : string) (l : list (value * value)) :=
+      NoDup (List.map fst l) /\
+        Forall (fun p => match snd p with
+                         | VRecord r =>
+                             match access_record r "0" with
+                             | Success (VList l) =>
+                                 Forall (fun r => match r with
+                                              | VRecord r => access_record r attr = Success (fst p)
+                                              | _ => False
+                                                  end) l
+                             | _ => False
+                             end /\
+                               match access_record r "1" with
+                               | Success (VRecord r) => access_record r attr = Success (fst p)
+                               | _ => False
+                               end
+                         | _ => False
+                         end) l.
+
+      Lemma index_wf_step_inv : forall attr p idx,
+          index_wf attr (p :: idx) -> index_wf attr idx.
+      Proof.
+        intros * H. destruct H as [HL HR]; inversion HL; inversion HR; subst.
+        split; auto.
       Qed.
 
       Lemma dict_lookup__filter_none : forall attr k idx,
@@ -1319,104 +1455,481 @@ Section WithWord.
           dict_lookup k idx = None ->
           gallina_filter_access_eq attr k (gallina_idx_to_list idx) = nil.
       Proof.
-        unfold gallina_filter_access_eq.
-        intros. induction idx; simpl; auto. destruct a; simpl in *. destruct v0; auto.
-        rewrite filter_app. destruct H as [HL HR]; inversion HL; inversion HR; subst.
-        destruct (value_eqb k v) eqn:E.
-        1: congruence.
+        unfold gallina_filter_access_eq, record_proj.
+        intros. induction idx; simpl; auto. unfold record_proj.
+        destruct a; simpl in *. destruct v1; auto.
+        destruct H as [HL HR]; inversion HL; inversion HR; subst; simpl in *.
+        destruct (access_record l "0"); intuition; destruct a; intuition.
+        destruct (access_record l "1"); intuition; destruct a; intuition.
+        rewrite filter_app. destruct (value_eqb k0 v0) eqn:E.
+        1: congruence. simpl.
         rewrite IHidx; auto. 2: split; auto.
-        rewrite app_nil_r. simpl in *. induction H6; simpl; auto. rewrite IHForall.
-        1:{ destruct x; intuition.
-            erewrite access_record__record_proj; eauto. rewrite value_eqb_sym. rewrite E; trivial. }
-        constructor; auto.
+        rewrite H1, value_eqb_sym, E, app_nil_r.
+        induction H; simpl; auto. rewrite IHForall.
+        destruct x; intuition. rewrite H, value_eqb_sym, E. reflexivity.
       Qed.
 
-      Lemma Forall_false__filter : forall A f (l : list A), Forall (fun x => f x = false) l -> filter f l = nil.
+      Lemma not_In__dict_lookup : forall (v : value) d, ~ In v (List.map fst d) -> dict_lookup v d = None.
       Proof.
-        intros * H; induction l; simpl; auto. simpl in H.
-        inversion H; subst. rewrite H2. auto.
+        intros * H. induction d; simpl; auto.
+        destruct a; simpl in *. intuition. destruct_match_goal; auto.
+        apply value_eqb_eq in E; subst; intuition.
       Qed.
 
-      Lemma In_gallina_idx_to_list : forall r idx,
-          In r (gallina_idx_to_list idx) -> exists k v, In (k, VList v) idx /\ In r v.
-      Proof.
-        intros. induction idx; simpl in *; intuition.
-        destruct a; simpl in *. destruct v0 eqn:E; try apply in_nil in H; intuition.
-        apply in_app_or in H; intuition.
-        - exists v; exists l; intuition.
-        - destruct H as [k' [v' H]]. exists k'; exists v'. intuition.
-      Qed.
-
-      Lemma dict_lookup__filter_some : forall attr k idx l,
+      Lemma dict_lookup__filter_some : forall attr k idx l v,
           index_wf attr idx ->
-          dict_lookup k idx = Some (VList l) ->
-          gallina_filter_access_eq attr k (gallina_idx_to_list idx) = l.
+          dict_lookup k idx = Some (VRecord [("0", VList l); ("1", v)]) ->
+          gallina_filter_access_eq attr k (gallina_idx_to_list idx) = (l ++ [v])%list.
       Proof.
-        unfold gallina_filter_access_eq.
-        intros; generalize dependent l; induction idx; simpl; intros.
-        1: congruence.
-        destruct H as [HL HR]; inversion HL; inversion HR; subst.
-        destruct a; simpl in *. destruct v0; intuition. rewrite filter_app.
-        destruct (value_eqb k v) eqn:E; auto.
-        2:{ erewrite IHidx; eauto. 2: split; auto.
-            lazymatch goal with |- ?l0 ++ _ = _ => replace l0 with (@nil value) end; auto.
-            induction l0; simpl; auto. inversion H6; subst. rewrite <- IHl0; auto.
-            destruct a; intuition.
-            erewrite access_record__record_proj; eauto. rewrite value_eqb_sym. rewrite E; trivial. }
-        1:{ injection H0; intros; subst.
-            rewrite forallb_filter_id.
-            1: lazymatch goal with |- _ ++ ?l = _ => replace l with (@nil value) end.
-            1: apply app_nil_r.
-            1:{ symmetry. apply Forall_false__filter. rewrite Forall_forall; intros r H_r_in.
-                apply In_gallina_idx_to_list in H_r_in as [k' [v' [H_in_L H_in_R]]].
-                apply_Forall_In. simpl in *. apply_Forall_In.
-                destruct r; intuition. erewrite access_record__record_proj; eauto.
-                destruct (value_eqb k' k) eqn:E'; auto. apply value_eqb_eq in E', E; subst.
-                apply in_map with (f:=fst) in H_in_L; simpl in *. intuition. }
-            rewrite forallb_forall; intros r H_in. apply_Forall_In. destruct r; intuition.
-            erewrite access_record__record_proj; eauto using value_eqb_sym. }
+        intros * H_wf H_lookup. induction idx; simpl in *; try congruence.
+        destruct a; simpl in *. destruct_match.
+        all: inversion H_wf; subst; invert_Forall.
+        1:{ do_injection; unfold record_proj; simpl. unfold gallina_filter_access_eq.
+            apply value_eqb_eq in E; subst. rewrite filter_app. f_equal.
+            1:{ apply forallb_filter_id. rewrite forallb_forall. intros x H_in.
+                simpl in *; intuition. apply_Forall_In. destruct x; intuition.
+                unfold record_proj. rewrite_l_to_r. apply value_eqb_refl. }
+            1:{ simpl in *; destruct v0; intuition. unfold record_proj. rewrite_l_to_r. rewrite value_eqb_refl.
+                f_equal. apply dict_lookup__filter_none. 1: eapply index_wf_step_inv; eauto.
+                apply not_In__dict_lookup. inversion H; auto. } }
+        1:{ simpl in *. destruct v2; intuition.
+            unfold record_proj. repeat destruct_match; intuition.
+            rewrite List.assoc_app_cons. unfold gallina_filter_access_eq. rewrite filter_app.
+            lazymatch goal with |- _ = ?x => replace x with (app nil x) end; auto.
+            f_equal. 2: rewrite <- IHidx; auto; eapply index_wf_step_inv; eauto.
+            apply Forall_false__filter. apply Forall_app. split.
+            1:{ rewrite Forall_forall. intros x H_in. apply_Forall_In. unfold record_proj.
+                destruct x; intuition. rewrite_l_to_r. rewrite value_eqb_sym; auto. }
+            1:{ constructor; auto. unfold record_proj; rewrite_l_to_r. rewrite value_eqb_sym; auto. } }
       Qed.
 
-    Lemma eq_filter_to_lookup_head_preserve_sem : forall tbl attr e (Gstore Genv : tenv) (store env : locals) rt t idx,
+      Lemma eq_filter_to_lookup_head_preserve_sem : forall tbl attr e (Gstore Genv : tenv) (store env : locals) rt t idx,
+          nodup_vars ->
+          tenv_wf Gstore -> tenv_wf Genv ->
+          map.get Gstore tbl = Some (index_type (get_attr_type rt attr) rt) ->
+          In attr (List.map fst rt) ->
+          type_of Gstore Genv e t ->
+          locals_wf Gstore store -> locals_wf Genv env ->
+          map.get store tbl = Some (VDict idx) ->
+          index_wf attr idx ->
+          interp_expr store env e = interp_expr store env (eq_filter_to_lookup_head tbl attr e).
+      Proof.
+        intros * vars_distinct H_Gstr H_Genv H_tbl_ty H_in H_ty H_str H_env H_tbl_v H_index_wf.
+        repeat destruct_subexpr. unfold eq_filter_to_lookup_head.
+        lazymatch goal with |- context[if ?x then _ else _] => destruct x eqn:E end; auto.
+        repeat rewrite Bool.andb_true_r in *. simpl in E.
+        repeat rewrite Bool.andb_true_iff in E; intuition. rewrite Bool.negb_true_iff, eqb_eq, eqb_neq in *; subst.
+        rewrite fold_idx_to_list.
+        repeat invert_type_of. repeat rewrite_map_get_put_hyp.
+        repeat (clear_refl; repeat do_injection).
+        erewrite fiat2_gallina_filter_access_eq; auto.
+        2: eapply fiat2_gallina_idx_to_list with (Gstore:=Gstore); eauto; simpl; intuition.
+        2: econstructor; eauto.
+        2: simpl; unfold get_local; rewrite H_tbl_v; auto.
+        eapply TyELoc in H_tbl_ty as H_tbl_ty'. apply_type_sound (ELoc tbl). simpl in H'. rewrite <- H1 in H'.
+        unfold get_local in H1. rewrite H_tbl_v in H1. injection H1; intros; subst.
+        specialize (dict_lookup_sound (width:=width) idx) as H_lookup.
+        eapply (H_lookup (get_attr_type rt attr) _ (interp_expr store env e2_2)) in H'; eauto.
+        2:{ unfold get_attr_type. lazymatch goal with
+              H: ?x = _, H': ?x = _ |- _ => rewrite H in H'
+              end. repeat (clear_refl; repeat do_injection).
+            simpl in *; repeat do_injection. rewrite H8; auto.
+            apply not_free_immut_put_ty in H10; auto. eapply type_sound; eauto. }
+        simpl. unfold get_local. rewrite H_tbl_v. inversion H'; subst.
+        2: rewrite map.get_put_same.
+        (* dict_lookup found no match *)
+        1: f_equal; auto using dict_lookup__filter_none.
+        (* dict_lookup found some match *)
+        1:{ invert_type_of_value. repeat invert_Forall2.
+            destruct x0, x1; intuition; simpl in *; subst.
+            unfold record_proj; simpl. invert_type_of_value. f_equal.
+            apply dict_lookup__filter_some; congruence. }
+      Qed.
+    End eq_filter_to_lookup.
+
+      Notation elist_to_idx tup0 tup1 tup2 tup3 tup4 acc0 acc1 acc2 x0 x1 x2 attr0 attr1 d :=
+        (EFold d (EDict []) tup0 acc0
+           (EInsert (EVar acc1) (EAccess (EVar tup1) attr0) (EOptMatch (ELookup (EVar acc2) (EAccess (EVar tup2) attr1)) (ERecord [("0", EAtom (ANil None)); ("1", EVar tup3)]) x0 (ERecord [("0", EBinop OCons (EVar tup4) (EAccess (EVar x1) "0")); ("1", EAccess (EVar x2) "1")] )))).
+
+      Notation eidx_to_list k v0 v1 v2 acc0 acc1 d :=
+        (EDictFold d (EAtom (ANil None)) k v0 acc0 (EBinop OConcat (EAccess (EVar v1) "0") (EBinop OCons (EAccess (EVar v2) "1") (EVar acc1)))).
+
+      Notation efilter x0 x1 attr0 k l :=
+        (EFilter l x0 (EUnop ONot (EBinop OEq (EAccess (EVar x1) attr0) k))).
+
+    Section neq_filter_to_delete.
+      Context (k v acc tup x : string).
+
+      Definition neq_filter_to_delete_head (tbl attr : string) (e : expr) :=
+        (* list_to_idx (filter (idx_to_list idx) (fun row => row.attr != e)) = delete idx e *)
+        match e with
+        | elist_to_idx tup0 tup1 tup2 tup3 tup4 acc0 acc1 acc2 x0 x1 x2 attr0 attr1
+            ((efilter y0 y1 attr2 k' (eidx_to_list k0 v0 v1 v2 acc3 acc4 (ELoc tbl0))))
+  => if (all_eqb [(tbl, [tbl0]); (k,[k0]); (v,[v0; v1; v2]); (acc, [acc0; acc1; acc2; acc3; acc4]); (y0, [y1]); (tup, [tup0; tup1; tup2; tup3; tup4]); (attr, [attr0; attr1; attr2]); (x, [x0; x1; x2])] && negb (free_immut_in y0 k'))%bool
+             then EDelete (ELoc tbl) k'
+             else e
+        | _ => e
+        end.
+
+(*
+      Definition neq_filter_to_delete_head (tbl attr : string) (e : expr) :=
+        (* list_to_idx (filter (idx_to_list idx) (fun row => row.attr != e)) = delete idx e *)
+        match e with
+        | (EFold
+             (EFilter
+                (EDictFold (ELoc tbl0) (EAtom (ANil None)) k0 v0 acc0 (EBinop OConcat (EAccess (EVar v1) "0") (EBinop OCons (EAccess (EVar v2) s1_0) (EVar acc1))))
+                y0 (EUnop ONot (EBinop OEq (EAccess (EVar y1) attr0) k')))
+             (EDict []) tup0 acc2
+             (EInsert (EVar acc3) (EAccess (EVar tup1) attr1) (EOptMatch (ELookup (EVar acc4) (EAccess (EVar tup2) attr2)) (ERecord [(s0_1, EAtom (ANil None)); (s1_1, EVar tup3)]) x0 (ERecord [(s0_2, EBinop OCons (EVar tup4) (EAccess (EVar x1) s0_3)); (s1_2, EAccess (EVar x2) s1_3)] ))))
+             => if (all_eqb [(tbl, [tbl0]); (k,[k0]); (v,[v0; v1; v2]); (acc, [acc0; acc1; acc2; acc3; acc4]); (y0, [y1]); (tup, [tup0; tup1; tup2; tup3; tup4]); (attr, [attr0; attr1; attr2]); (x, [x0; x1; x2]); ("0", [s0_1; s0_2; s0_3]); ("1", [s1_0; s1_1; s1_2; s1_3])] && negb (free_immut_in y0 k'))%bool
+             then EDelete (ELoc tbl) k'
+             else e
+        | _ => e
+        end.
+*)
+    Definition gallina_filter_access_neq (s : string) (v0 : value) (l : list value) :=
+      filter (fun v => negb (value_eqb match v with
+                         | VRecord r => record_proj s r
+                         | _ => VUnit
+                         end v0)) l.
+
+    Lemma fiat2_gallina_filter_access_neq :
+      forall (store env : locals) e1 e2 x s l,
+        interp_expr store env e1 = VList l ->
+        free_immut_in x e2 = false ->
+        interp_expr store env (EFilter e1 x (EUnop ONot (EBinop OEq (EAccess (EVar x) s) e2))) =
+          VList (gallina_filter_access_neq s (interp_expr store env e2) l).
+      Proof.
+        intros * H1 H_free; simpl. rewrite H1. f_equal. apply filter_ext. intro a.
+        unfold get_local. rewrite map.get_put_same. rewrite <- not_free_immut_put_sem; auto.
+      Qed.
+
+      Lemma neq_filter_to_delete_head_preserve_ty : forall tbl attr (e : expr) rt t (Gstore Genv : tenv),
+          is_NoDup [v; acc; tup; x] ->
+          tenv_wf Gstore ->
+          tenv_wf Genv ->
+          map.get Gstore tbl = Some (index_type (get_attr_type rt attr) rt) ->
+          type_of Gstore Genv e t ->
+          type_of Gstore Genv (neq_filter_to_delete_head tbl attr e) t.
+      Proof.
+        intros * vars_distinct H_Gstr H_Genv H_tbl_ty H_ty.
+        repeat destruct_subexpr. simpl. destruct_match_goal; auto.
+        repeat rewrite Bool.andb_true_r in E. repeat rewrite Bool.andb_true_iff in E; intuition.
+        rewrite Bool.negb_true_iff, eqb_eq in *; subst.
+        repeat invert_type_of. repeat rewrite_map_get_put_hyp. repeat (clear_refl; repeat do_injection).
+        repeat constructor; auto.
+        1:{ lazymatch goal with
+            H: map.get Gstore tbl = _, H': map.get Gstore tbl = _ |- _ =>
+              rewrite H in *; do_injection; simpl in *; do_injection
+          end.
+            unfold get_attr_type. rewrite H23.
+            do 3 (destruct tl; simpl in *; try congruence). destruct p, p0; simpl in *; injection H1; intros; subst.
+            assert ([("0", t); ("1", t0)] = tl').
+            { apply Permutation_length_2_inv in H4; destruct H4; auto. subst; inversion H19; subst. inversion H7; subst.
+              unfold record_entry_leb in H10; inversion H10. }
+            inversion H2; subst. inversion H13; subst. repeat invert_type_of. repeat rewrite_map_get_put_hyp. repeat (clear_refl; do_injection).
+            unfold index_type. apply Permutation_sym, Permutation_length_2_inv in H17. destruct H17; subst.
+            all: inversion H15; subst; inversion H12; subst; repeat invert_type_of; repeat rewrite_map_get_put_hyp. do_injection. auto. }
+        1:{ repeat lazymatch goal with
+              H: ?x = _, H': ?x = _ |- _ => rewrite H in H'
+              end. repeat (clear_refl; repeat do_injection).
+            eapply not_free_immut_put_ty; eauto. }
+      Qed.
+
+      Lemma fold_list_to_idx : forall tup acc x attr tbl,
+          EFold tbl (EDict []) tup acc
+            (EInsert (EVar acc) (EAccess (EVar tup) attr)
+               (EOptMatch (ELookup (EVar acc) (EAccess (EVar tup) attr))
+                  (epair enil (EVar tup)) x (cons_to_fst (EVar tup) (EVar x)))) =
+            list_to_idx tup acc x attr tbl.
+    Proof. reflexivity. Qed.
+
+    Lemma dict_insert_Lt : forall k (v : value) d,
+                    (forall p, In p d -> value_compare k (fst p) = Lt) ->
+                    dict_insert k v d = (k, v) :: d.
+    Proof.
+      destruct d; simpl; auto; intros.
+      repeat destruct_match_goal; auto.
+      all: lazymatch goal with
+             H: forall _, (?k, ?v) = _ \/ _ -> _ |- _ => specialize H with (k, v)
+           end;
+        simpl in *; intuition.
+      1:{ lazymatch goal with
+          H: value_eqb _ _ = true |- _ => apply value_eqb_eq in H; subst
+        end.
+          rewrite value_compare_refl in *; congruence. }
+      1:{ unfold value_ltb in *.
+          lazymatch goal with
+            H: context[match ?x with _ => _ end], E: ?x = _ |- _ => rewrite E in H
+          end. congruence. }
+    Qed.
+
+    Local Ltac invert_NoDup :=
+      lazymatch goal with H: NoDup (_ :: _) |- _ => inversion H; subst; clear H end.
+
+    Lemma NoDup_SSorted__Lt : forall (k v : value) d,
+        NoDup (k :: List.map fst d) ->
+        StronglySorted dict_entry_leb ((k, v) :: d) ->
+        forall p, In p d -> value_compare k (fst p) = Lt.
+    Proof.
+      intros. invert_NoDup; invert_SSorted. destruct p; simpl.
+      apply_Forall_In; unfold dict_entry_leb in *; simpl in *.
+      unfold value_leb, leb_from_compare in *.
+      lazymatch goal with |- ?x = _ => destruct x eqn:E end; try congruence.
+      apply value_compare_Eq_eq in E; subst. apply in_map with (f:=fst) in H1; intuition.
+    Qed.
+
+    Lemma gallina_idx_to_list_to_idx : forall attr idx kt rt,
+        type_of_value (VDict idx) (index_type kt rt) ->
+        index_wf attr idx -> gallina_list_to_idx attr (gallina_idx_to_list idx) = idx.
+    Proof.
+      intros * H_ty H_wf. induction idx; simpl; auto.
+      apply index_wf_step_inv in H_wf as H_wf'.
+      destruct a as [k0 v0]; simpl.
+      destruct H_wf as [HL HR]. inversion HL; inversion HR; subst.
+      destruct v0; simpl in *; intuition. unfold record_proj. repeat destruct_match; intuition.
+
+      unfold gallina_list_to_idx in *. rewrite List.assoc_app_cons, fold_right_app. rewrite IHidx; auto.
+      all: inversion H_ty; subst; invert_Forall; invert_SSorted; subst. 2: constructor; intuition.
+      generalize dependent l; induction l1; intros; simpl in *; auto.
+      all: intuition; inversion H4; subst; repeat invert_Forall2.
+      all: destruct x0, x1; simpl in *; intuition; subst.
+      1:{ unfold record_proj; lazymatch goal with H: ?x = Success _ |- context[?x] => rewrite H end.
+          rewrite dict_lookup_Lt; eauto using NoDup_SSorted__Lt.
+          rewrite dict_insert_Lt; eauto using NoDup_SSorted__Lt; congruence. }
+      1:{ destruct v0; simpl in *; try congruence. destruct l; try congruence.
+          rewrite IHl1 with (l:=[("0", VList l); ("1", v1)]); simpl; auto; try congruence.
+          all: repeat invert_Forall; intuition.
+          all: repeat (constructor; simpl in *; auto);
+            lazymatch goal with H: type_of_value (VList (_ :: ?l)) _ |- _ => inversion H; subst end;
+            invert_Forall; intuition.
+          2: invert_Forall; auto.
+          destruct_match_goal; intuition. unfold record_proj. rewrite_l_to_r.
+          unfold value_ltb, value_eqb. rewrite value_compare_refl.
+          unfold vcons_to_fst, record_proj; simpl. congruence. }
+    Qed.
+
+    Lemma not_In__dict_delete : forall (k : value) d, ~ In k (List.map fst d) -> dict_delete k d = d.
+    Proof.
+      induction d; intros; simpl; auto.
+      destruct a; destruct_match_goal; simpl in *.
+      1:apply value_eqb_eq in E; subst; intuition.
+      f_equal. auto.
+    Qed.
+
+    Lemma gallina_filter_access_neq_idx_to_list : forall attr k idx,
+                 index_wf attr idx ->
+                 gallina_filter_access_neq attr k (gallina_idx_to_list idx) = gallina_idx_to_list (dict_delete k idx).
+    Proof.
+      intros * H. induction idx; auto.
+      simpl. inversion H; invert_Forall. destruct_match; intuition; simpl in *.
+      repeat destruct_match; intuition. unfold record_proj; repeat rewrite_l_to_r.
+      destruct a; simpl in *.
+      unfold gallina_filter_access_neq in *. rewrite filter_app. simpl. rewrite IHidx.
+      2: eapply index_wf_step_inv; eauto.
+      destruct (value_eqb k0 v0) eqn:E_k0v0.
+      1:{ apply value_eqb_eq in E_k0v0; subst. unfold record_proj; rewrite_l_to_r. rewrite value_eqb_refl; simpl.
+          rewrite not_In__dict_delete. 2: invert_NoDup; auto.
+          rewrite Forall_false__filter; auto. rewrite Forall_forall; intros. apply_Forall_In.
+          destruct_match; intuition. rewrite_l_to_r. rewrite value_eqb_refl; auto. }
+      1:{ simpl. unfold record_proj; rewrite value_eqb_sym; repeat rewrite_l_to_r. simpl.
+          f_equal. apply forallb_filter_id. rewrite forallb_forall; intros; apply_Forall_In.
+          destruct_match; intuition. rewrite_l_to_r. rewrite value_eqb_sym. rewrite_l_to_r; auto. }
+    Qed.
+
+    Lemma dict_delete_preserve_index_wf : forall attr idx,
+        index_wf attr idx ->
+        forall k, index_wf attr (dict_delete k idx).
+    Proof.
+      intros * H_wf *.
+      induction idx; simpl; auto.
+      destruct a. destruct (value_eqb k0 v0).
+      all: apply index_wf_step_inv in H_wf as H_wf'; auto.
+      specialize (IHidx H_wf').
+      destruct H_wf as [HL HR]; inversion HL; inversion HR; subst.
+      unfold index_wf; simpl; intuition.
+      1:{ constructor. 1: apply dict_delete_preserve_NoDup; auto. apply IHidx; auto. }
+      1:{ constructor; auto. eapply incl_Forall; eauto. apply dict_delete_incl. }
+    Qed.
+
+    Lemma neq_filter_to_delete_head_preserve_sem : forall tbl attr e (Gstore Genv : tenv) (store env : locals) rt t idx,
+        is_NoDup [v; acc; tup; x] ->
         tenv_wf Gstore -> tenv_wf Genv ->
-        map.get Gstore tbl = Some (TDict (get_attr_type rt attr) (TList (TRecord rt))) ->
+        map.get Gstore tbl = Some (index_type (get_attr_type rt attr) rt) ->
         In attr (List.map fst rt) ->
         type_of Gstore Genv e t ->
         locals_wf Gstore store -> locals_wf Genv env ->
         map.get store tbl = Some (VDict idx) ->
         index_wf attr idx ->
-        interp_expr store env e = interp_expr store env (eq_filter_to_lookup_head tbl attr e).
+        interp_expr store env e = interp_expr store env (neq_filter_to_delete_head tbl attr e).
     Proof.
-      intros * H_Gstr H_Genv H_tbl_ty H_in H_ty H_str H_env H_tbl_v H_index_wf.
-      (* ??? How to automate this? *)
-      destruct e; auto. destruct e1; auto. destruct e1_1; auto. destruct e1_2; auto.
-      destruct a; auto. destruct t0; auto. destruct e1_3; auto. destruct o; auto.
-      destruct e1_3_1; auto. destruct e1_3_2; auto. destruct e2; auto. destruct o; auto.
-      destruct e2_1; auto. destruct e2_1; auto.
-      unfold eq_filter_to_lookup_head.
-      lazymatch goal with |- context[if ?x then _ else _] => destruct x eqn:E end; auto.
-      repeat rewrite Bool.andb_true_iff in E; intuition. rewrite Bool.negb_true_iff, eqb_eq, eqb_neq in *; subst.
-      fold (idx_to_list (ELoc tbl)).
-      repeat invert_type_of. repeat rewrite_map_get_put.
-      repeat (clear_refl; repeat do_injection).
-      erewrite fiat2_gallina_filter_access_eq; auto.
-      2: eapply fiat2_gallina_idx_to_list with (Gstore:=Gstore); eauto.
-      2: econstructor; eauto.
-      2: simpl; unfold get_local; rewrite H_tbl_v; auto.
-      eapply TyELoc in H_tbl_ty as H_tbl_ty'. apply_type_sound (ELoc tbl). simpl in H'. rewrite <- H1 in H'.
-      unfold get_local in H1. rewrite H_tbl_v in H1. injection H1; intros; subst.
-      specialize (dict_lookup_sound (width:=width) idx) as H_lookup.
-      eapply (H_lookup (get_attr_type rt attr) (TList (TRecord rt)) (interp_expr store env e2_2)) in H'; eauto.
-      2:{ unfold get_attr_type. rewrite H_tbl_ty in H10. repeat (clear_refl; repeat do_injection). rewrite H7; auto.
-          apply not_free_immut_put_ty in H9; auto. eapply type_sound in H9; eauto. }
-      simpl. unfold get_local. rewrite H_tbl_v. inversion H'; subst.
-      2: rewrite map.get_put_same.
-      (* dict_lookup found no match *)
-      1: f_equal; auto using dict_lookup__filter_none.
-      (* dict_lookup found some match *)
-      1:{ lazymatch goal with H: type_of_value ?v _ |- _ = ?v => inversion H; subst end. f_equal.
-          apply dict_lookup__filter_some; auto. }
+      intros * vars_distinct H_Gstr H_Genv H_tbl_ty H_in H_ty H_str H_env H_tbl_v H_index_wf.
+      repeat destruct_subexpr. unfold neq_filter_to_delete_head. destruct_match_goal; auto.
+      simpl in E. repeat rewrite Bool.andb_true_r in E.
+      repeat rewrite Bool.andb_true_iff in E; intuition. rewrite Bool.negb_true_iff, eqb_eq in *; subst.
+      rewrite fold_idx_to_list, fold_list_to_idx in *.
+      erewrite fiat2_gallina_list_to_idx with (Gstore:=Gstore); eauto.
+      2: simpl in *; intuition.
+      3:{ erewrite fiat2_gallina_filter_access_neq; auto. eapply fiat2_gallina_idx_to_list with (Gstore:=Gstore); eauto.
+          1: simpl in *; intuition.
+          1: econstructor; eauto.
+          1: simpl; unfold get_local; rewrite H_tbl_v; eauto. }
+      2:{ repeat invert_type_of. repeat rewrite_map_get_put_hyp; repeat (clear_refl; repeat do_injection).
+          repeat (constructor; auto).
+          1: eapply idx_to_list_preserve_ty; eauto; constructor; eauto; simpl in *; intuition.
+          lazymatch goal with
+            H: ?x = _, H': ?x = _ |- _ => rewrite H in H'
+          end; do_injection; auto. simpl in *; do_injection.
+          repeat (econstructor; eauto). rewrite_map_get_put_goal; auto. }
+      simpl. unfold get_local. rewrite H_tbl_v. f_equal.
+      erewrite gallina_filter_access_neq_idx_to_list, gallina_idx_to_list_to_idx; auto using dict_delete_preserve_index_wf.
+      apply dict_delete_sound. 3: specialize (H_str _ _ H_tbl_ty); rewrite H_tbl_v in H_str; eauto.
+      all: repeat invert_type_of; repeat rewrite_map_get_put_hyp; repeat (clear_refl; repeat do_injection).
+      all: repeat lazymatch goal with
+               H: ?x = _, H': ?x = _ |- _ => rewrite H in H'
+             end; [> do_injection ..]; simpl in *; repeat (clear_refl; repeat do_injection).
+      1: apply get_attr_type_ty_wf; auto.
+      1:{ constructor; simpl.
+          1: repeat constructor. 1: rewrite <- inb_false_iff; auto. 1: intuition.
+          1: repeat constructor. repeat (constructor; auto). }
+      lazymatch goal with
+        H: type_of _ _ ?e _ |- context[?e] =>
+          apply not_free_immut_put_ty in H; auto; eapply type_sound in H; eauto
+      end.
+      unfold get_attr_type. rewrite_l_to_r; auto.
     Qed.
+    End neq_filter_to_delete.
+
+    Section cons_to_insert.
+      Context (k v acc tup x y : string).
+
+      Definition cons_to_insert_head (tbl attr : string) (e : expr) :=
+        (* list_to_idx (cons e (idx_to_list idx)) = insert idx (e.attr) (e :: lookup idx e.attr) *)
+        match e with
+        | elist_to_idx tup0 tup1 tup2 tup3 tup4 acc0 acc1 acc2 x0 x1 x2 attr0 attr1
+            (EBinop OCons row (eidx_to_list k0 v0 v1 v2 acc3 acc4 (ELoc tbl0))) =>
+             if (all_eqb [(tbl, [tbl0]); (k,[k0]); (v, [v0; v1; v2]); (acc, [acc0; acc1; acc2; acc3; acc4]); (tup, [tup0; tup1; tup2; tup3; tup4]); (attr, [attr0; attr1]); (x, [x0; x1; x2])] && negb (free_immut_in y row))%bool
+             then EInsert (ELoc tbl) (EAccess row attr)
+                       (EOptMatch (ELookup (ELoc tbl) (EAccess row attr)) (epair enil row) y (cons_to_fst row (EVar y)))
+             else e
+        | _ => e
+        end.
+
+      Lemma not_free_immut_put_ty_inv : forall (x : string) (e : expr) (Gstore Genv : tenv) (t t' : type),
+          free_immut_in x e = false -> type_of Gstore Genv e t -> type_of Gstore (map.put Genv x t') e t.
+      Proof.
+        intros * H_free H. induction H using @type_of_IH.
+        - (* EVar *)
+          constructor; simpl in *; rewrite_map_get_put_goal. symmetry. apply eqb_neq; auto.
+        - (* ELoc *)
+          constructor; auto.
+        - (* EAtom *)
+          constructor; auto.
+        - (* EUnop *) admit.
+          Admitted.
+
+      Lemma cons_to_insert_head_preserve_ty : forall tbl attr (e : expr) rt t (Gstore Genv : tenv),
+          is_NoDup [tup; acc; v; x] ->
+          tenv_wf Gstore ->
+          tenv_wf Genv ->
+          map.get Gstore tbl = Some (index_type (get_attr_type rt attr) rt) ->
+          type_of Gstore Genv e t ->
+          type_of Gstore Genv (cons_to_insert_head tbl attr e) t.
+      Proof.
+        intros * vars_distinct H_Gstr H_Genv H_tbl_ty H_ty.
+        repeat destruct_subexpr. simpl; auto.
+        destruct_match_goal; auto. repeat rewrite Bool.andb_true_r in E.
+        repeat rewrite Bool.andb_true_iff in E; intuition. rewrite eqb_eq, Bool.negb_true_iff in *; subst.
+        repeat invert_type_of. repeat rewrite_map_get_put_hyp. repeat (try clear_refl; repeat do_injection); auto.
+        repeat (econstructor; eauto).
+        all: repeat invert_Forall2; simpl in *; repeat invert_type_of;
+          repeat rewrite_map_get_put_hyp; repeat (try clear_refl; repeat do_injection).
+        1:{ lazymatch goal with
+             H: map.get Gstore tbl = _, H': map.get Gstore tbl = _ |- _=>
+               rewrite H in H'; repeat do_injection; rewrite H; repeat f_equal end.
+            simpl in *. repeat (try clear_refl; repeat do_injection).
+            unfold get_attr_type, index_type. rewrite_l_to_r.
+            do 3 (destruct tl; simpl in *; try congruence).
+            do 3 (destruct tl1; simpl in *; try congruence).
+            lazymatch goal with
+            | H: Permutation _ _ |- _ =>
+                apply Permutation_length_2_inv in H; destruct H; subst
+            end.
+            2:{ invert_SSorted. lazymatch goal with H: Forall _ [_] |- _ => inversion H; subst end.
+                unfold record_entry_leb in *.
+                repeat lazymatch goal with H: ["0"; "1"] = [_; _] |- _ => inversion H; subst; clear H end.
+                lazymatch goal with
+                  H1: _ = fst p1, H2: _ = fst p2 |- _ =>
+                    rewrite <- H1, <- H2 in *
+                end. inversion H13. }
+            repeat lazymatch goal with
+                     H: _ :: _ = _ :: _ |- _ => inversion H; subst; clear H end.
+            destruct p, p0, p1, p2; simpl in *.
+            repeat lazymatch goal with
+                   | H: "0" = _ |- _ => rewrite <- H in *; clear H
+                   | H: "1" = _ |- _ => rewrite <- H in *; clear H
+                   end.
+            congruence. }
+        1:{ lazymatch goal with
+             H: map.get Gstore tbl = _, H': map.get Gstore tbl = _ |- _=>
+               rewrite H in H'; repeat do_injection end.
+            simpl in *; do_injection. unfold get_attr_type. rewrite_l_to_r; auto. }
+        1: repeat constructor; auto.
+        1:{ do 3 (destruct tl; simpl in *; try congruence).
+            do 3 (destruct tl1; simpl in *; try congruence).
+            lazymatch goal with
+            | H: Permutation _ _ |- _ =>
+                apply Permutation_length_2_inv in H; destruct H; subst
+            end.
+            2:{ invert_SSorted. lazymatch goal with H: Forall _ [_] |- _ => inversion H; subst end.
+                unfold record_entry_leb in *.
+                repeat lazymatch goal with H: ["0"; "1"] = [_; _] |- _ => inversion H; subst; clear H end.
+                lazymatch goal with
+                  H1: _ = fst p1, H2: _ = fst p2 |- _ =>
+                    rewrite <- H1, <- H2 in *
+                end. inversion H13. }
+            repeat lazymatch goal with
+                     H: _ :: _ = _ :: _ |- _ => inversion H; subst; clear H end.
+            destruct p, p0, p1, p2; simpl in *.
+            repeat lazymatch goal with
+                   | H: "0" = _ |- _ => rewrite <- H in *; clear H
+                   | H: "1" = _ |- _ => rewrite <- H in *; clear H
+                   end. repeat (try clear_refl; repeat do_injection).
+            repeat (econstructor; eauto).
+            2,3: rewrite_map_get_put_goal; auto.
+            apply not_free_immut_put_ty_inv; auto. }
+      Qed.
+
+      Lemma cons_to_insert_head_preserve_sem : forall tbl attr e (Gstore Genv : tenv) (store env : locals) rt t idx,
+          tenv_wf Gstore -> tenv_wf Genv ->
+          map.get Gstore tbl = Some (index_type (get_attr_type rt attr) rt) ->
+          In attr (List.map fst rt) ->
+          type_of Gstore Genv e t ->
+          locals_wf Gstore store -> locals_wf Genv env ->
+          map.get store tbl = Some (VDict idx) ->
+          index_wf attr idx ->
+          interp_expr store env e = interp_expr store env (cons_to_insert_head tbl attr e).
+      Admitted.
+    End cons_to_insert.
+
+
+(***??? in construction ???***)
+
+    Lemma ESort_Permutation_inv : forall (store env : locals) l l' vl vl',
+        interp_expr store env l = VList vl ->
+        interp_expr store env l' = VList vl' ->
+        Permutation vl vl' ->
+        interp_expr store env (ESort l) = interp_expr store env (ESort l').
+    Proof.
+      intros store env l l' vl vl' E E' H. simpl.
+      rewrite E, E'. f_equal.
+      apply Permutation_SSorted_eq.
+      2,3: apply StronglySorted_value_sort.
+      eapply perm_trans. 2:apply Permuted_value_sort.
+      eapply perm_trans. 2:apply H.
+      apply Permutation_sym, Permuted_value_sort.
+    Qed.
+
   End WithMap.
 
   (* ??? TODO: to be moved *)
@@ -1447,7 +1960,7 @@ Section WithWord.
 
     Compute typecheck (map.put map.empty "res" TInt) map.empty ex1. *)
 
-    Definition ex1' := transf_to_idx "persons" "id" ex1.
+    Definition ex1' := transf_to_idx "tup" "acc" "x" "k" "v" "persons" "id" ex1.
 (*  Compute ex1'. *)
 
     Goal interp_command (map.put map.empty "res" (VInt 0)) (map.empty (value:=value)) ex1' = interp_command (map.put map.empty "res" (VInt 0)) map.empty ex1.
